src/ocaml/extraction/QFBV.mli
@@ -1398,6 +1398,1236 @@ module MakeQFBV :
   val string_of_exp : exp -> char list
 
   val string_of_bexp : bexp -> char list
+
+  module MA :
+   sig
+    module MA :
+     sig
+      module VSLemmas :
+       sig
+        module F :
+         sig
+          val eqb : Equality.sort -> Equality.sort -> bool
+         end
+
+        module OP :
+         sig
+          module ME :
+           sig
+            module TO :
+             sig
+              type t = Equality.sort
+             end
+
+            module IsTO :
+             sig
+             end
+
+            module OrderTac :
+             sig
+             end
+
+            val eq_dec : Equality.sort -> Equality.sort -> bool
+
+            val lt_dec : Equality.sort -> Equality.sort -> bool
+
+            val eqb : Equality.sort -> Equality.sort -> bool
+           end
+
+          module P :
+           sig
+            module Dec :
+             sig
+              module F :
+               sig
+                val eqb : Equality.sort -> Equality.sort -> bool
+               end
+
+              module FSetLogicalFacts :
+               sig
+               end
+
+              module FSetDecideAuxiliary :
+               sig
+               end
+
+              module FSetDecideTestCases :
+               sig
+               end
+             end
+
+            module FM :
+             sig
+              val eqb : Equality.sort -> Equality.sort -> bool
+             end
+
+            val coq_In_dec : VS.elt -> VS.t -> bool
+
+            val of_list : VS.elt list -> VS.t
+
+            val to_list : VS.t -> VS.elt list
+
+            val fold_rec :
+              (VS.elt -> 'a1 -> 'a1) -> 'a1 -> VS.t -> (VS.t -> __ -> 'a2) ->
+              (VS.elt -> 'a1 -> VS.t -> VS.t -> __ -> __ -> __ -> 'a2 -> 'a2)
+              -> 'a2
+
+            val fold_rec_bis :
+              (VS.elt -> 'a1 -> 'a1) -> 'a1 -> VS.t -> (VS.t -> VS.t -> 'a1
+              -> __ -> 'a2 -> 'a2) -> 'a2 -> (VS.elt -> 'a1 -> VS.t -> __ ->
+              __ -> 'a2 -> 'a2) -> 'a2
+
+            val fold_rec_nodep :
+              (VS.elt -> 'a1 -> 'a1) -> 'a1 -> VS.t -> 'a2 -> (VS.elt -> 'a1
+              -> __ -> 'a2 -> 'a2) -> 'a2
+
+            val fold_rec_weak :
+              (VS.elt -> 'a1 -> 'a1) -> 'a1 -> (VS.t -> VS.t -> 'a1 -> __ ->
+              'a2 -> 'a2) -> 'a2 -> (VS.elt -> 'a1 -> VS.t -> __ -> 'a2 ->
+              'a2) -> VS.t -> 'a2
+
+            val fold_rel :
+              (VS.elt -> 'a1 -> 'a1) -> (VS.elt -> 'a2 -> 'a2) -> 'a1 -> 'a2
+              -> VS.t -> 'a3 -> (VS.elt -> 'a1 -> 'a2 -> __ -> 'a3 -> 'a3) ->
+              'a3
+
+            val set_induction :
+              (VS.t -> __ -> 'a1) -> (VS.t -> VS.t -> 'a1 -> VS.elt -> __ ->
+              __ -> 'a1) -> VS.t -> 'a1
+
+            val set_induction_bis :
+              (VS.t -> VS.t -> __ -> 'a1 -> 'a1) -> 'a1 -> (VS.elt -> VS.t ->
+              __ -> 'a1 -> 'a1) -> VS.t -> 'a1
+
+            val cardinal_inv_2 : VS.t -> int -> VS.elt
+
+            val cardinal_inv_2b : VS.t -> VS.elt
+           end
+
+          val gtb : Equality.sort -> Equality.sort -> bool
+
+          val leb : Equality.sort -> Equality.sort -> bool
+
+          val elements_lt : Equality.sort -> VS.t -> Equality.sort list
+
+          val elements_ge : Equality.sort -> VS.t -> Equality.sort list
+
+          val set_induction_max :
+            (VS.t -> __ -> 'a1) -> (VS.t -> VS.t -> 'a1 -> Equality.sort ->
+            __ -> __ -> 'a1) -> VS.t -> 'a1
+
+          val set_induction_min :
+            (VS.t -> __ -> 'a1) -> (VS.t -> VS.t -> 'a1 -> Equality.sort ->
+            __ -> __ -> 'a1) -> VS.t -> 'a1
+         end
+
+        val eqb : Equality.sort -> Equality.sort -> bool
+
+        module ME :
+         sig
+          module TO :
+           sig
+            type t = Equality.sort
+           end
+
+          module IsTO :
+           sig
+           end
+
+          module OrderTac :
+           sig
+           end
+
+          val eq_dec : Equality.sort -> Equality.sort -> bool
+
+          val lt_dec : Equality.sort -> Equality.sort -> bool
+
+          val eqb : Equality.sort -> Equality.sort -> bool
+         end
+
+        module P :
+         sig
+          module Dec :
+           sig
+            module F :
+             sig
+              val eqb : Equality.sort -> Equality.sort -> bool
+             end
+
+            module FSetLogicalFacts :
+             sig
+             end
+
+            module FSetDecideAuxiliary :
+             sig
+             end
+
+            module FSetDecideTestCases :
+             sig
+             end
+           end
+
+          module FM :
+           sig
+            val eqb : Equality.sort -> Equality.sort -> bool
+           end
+
+          val coq_In_dec : VS.elt -> VS.t -> bool
+
+          val of_list : VS.elt list -> VS.t
+
+          val to_list : VS.t -> VS.elt list
+
+          val fold_rec :
+            (VS.elt -> 'a1 -> 'a1) -> 'a1 -> VS.t -> (VS.t -> __ -> 'a2) ->
+            (VS.elt -> 'a1 -> VS.t -> VS.t -> __ -> __ -> __ -> 'a2 -> 'a2)
+            -> 'a2
+
+          val fold_rec_bis :
+            (VS.elt -> 'a1 -> 'a1) -> 'a1 -> VS.t -> (VS.t -> VS.t -> 'a1 ->
+            __ -> 'a2 -> 'a2) -> 'a2 -> (VS.elt -> 'a1 -> VS.t -> __ -> __ ->
+            'a2 -> 'a2) -> 'a2
+
+          val fold_rec_nodep :
+            (VS.elt -> 'a1 -> 'a1) -> 'a1 -> VS.t -> 'a2 -> (VS.elt -> 'a1 ->
+            __ -> 'a2 -> 'a2) -> 'a2
+
+          val fold_rec_weak :
+            (VS.elt -> 'a1 -> 'a1) -> 'a1 -> (VS.t -> VS.t -> 'a1 -> __ ->
+            'a2 -> 'a2) -> 'a2 -> (VS.elt -> 'a1 -> VS.t -> __ -> 'a2 -> 'a2)
+            -> VS.t -> 'a2
+
+          val fold_rel :
+            (VS.elt -> 'a1 -> 'a1) -> (VS.elt -> 'a2 -> 'a2) -> 'a1 -> 'a2 ->
+            VS.t -> 'a3 -> (VS.elt -> 'a1 -> 'a2 -> __ -> 'a3 -> 'a3) -> 'a3
+
+          val set_induction :
+            (VS.t -> __ -> 'a1) -> (VS.t -> VS.t -> 'a1 -> VS.elt -> __ -> __
+            -> 'a1) -> VS.t -> 'a1
+
+          val set_induction_bis :
+            (VS.t -> VS.t -> __ -> 'a1 -> 'a1) -> 'a1 -> (VS.elt -> VS.t ->
+            __ -> 'a1 -> 'a1) -> VS.t -> 'a1
+
+          val cardinal_inv_2 : VS.t -> int -> VS.elt
+
+          val cardinal_inv_2b : VS.t -> VS.elt
+         end
+
+        val gtb : Equality.sort -> Equality.sort -> bool
+
+        val leb : Equality.sort -> Equality.sort -> bool
+
+        val elements_lt : Equality.sort -> VS.t -> Equality.sort list
+
+        val elements_ge : Equality.sort -> VS.t -> Equality.sort list
+
+        val set_induction_max :
+          (VS.t -> __ -> 'a1) -> (VS.t -> VS.t -> 'a1 -> Equality.sort -> __
+          -> __ -> 'a1) -> VS.t -> 'a1
+
+        val set_induction_min :
+          (VS.t -> __ -> 'a1) -> (VS.t -> VS.t -> 'a1 -> Equality.sort -> __
+          -> __ -> 'a1) -> VS.t -> 'a1
+
+        val memP : VS.elt -> VS.t -> reflect
+
+        val equalP : VS.t -> VS.t -> reflect
+
+        val subsetP : VS.t -> VS.t -> reflect
+
+        val emptyP : VS.t -> reflect
+
+        val disjoint : VS.t -> VS.t -> bool
+
+        val proper_subset : VS.t -> VS.t -> bool
+       end
+
+      module VMLemmas :
+       sig
+        module F :
+         sig
+          val eqb : Equality.sort -> Equality.sort -> bool
+
+          val coq_In_dec : 'a1 TE.t -> TE.key -> bool
+         end
+
+        module OP :
+         sig
+          module ME :
+           sig
+            module TO :
+             sig
+              type t = Equality.sort
+             end
+
+            module IsTO :
+             sig
+             end
+
+            module OrderTac :
+             sig
+             end
+
+            val eq_dec : Equality.sort -> Equality.sort -> bool
+
+            val lt_dec : Equality.sort -> Equality.sort -> bool
+
+            val eqb : Equality.sort -> Equality.sort -> bool
+           end
+
+          module O :
+           sig
+            module MO :
+             sig
+              module TO :
+               sig
+                type t = Equality.sort
+               end
+
+              module IsTO :
+               sig
+               end
+
+              module OrderTac :
+               sig
+               end
+
+              val eq_dec : Equality.sort -> Equality.sort -> bool
+
+              val lt_dec : Equality.sort -> Equality.sort -> bool
+
+              val eqb : Equality.sort -> Equality.sort -> bool
+             end
+           end
+
+          module P :
+           sig
+            module F :
+             sig
+              val eqb : Equality.sort -> Equality.sort -> bool
+
+              val coq_In_dec : 'a1 TE.t -> TE.key -> bool
+             end
+
+            val uncurry : ('a1 -> 'a2 -> 'a3) -> ('a1 * 'a2) -> 'a3
+
+            val of_list : (TE.key * 'a1) list -> 'a1 TE.t
+
+            val to_list : 'a1 TE.t -> (TE.key * 'a1) list
+
+            val fold_rec :
+              (TE.key -> 'a1 -> 'a2 -> 'a2) -> 'a2 -> 'a1 TE.t -> ('a1 TE.t
+              -> __ -> 'a3) -> (TE.key -> 'a1 -> 'a2 -> 'a1 TE.t -> 'a1 TE.t
+              -> __ -> __ -> __ -> 'a3 -> 'a3) -> 'a3
+
+            val fold_rec_bis :
+              (TE.key -> 'a1 -> 'a2 -> 'a2) -> 'a2 -> 'a1 TE.t -> ('a1 TE.t
+              -> 'a1 TE.t -> 'a2 -> __ -> 'a3 -> 'a3) -> 'a3 -> (TE.key ->
+              'a1 -> 'a2 -> 'a1 TE.t -> __ -> __ -> 'a3 -> 'a3) -> 'a3
+
+            val fold_rec_nodep :
+              (TE.key -> 'a1 -> 'a2 -> 'a2) -> 'a2 -> 'a1 TE.t -> 'a3 ->
+              (TE.key -> 'a1 -> 'a2 -> __ -> 'a3 -> 'a3) -> 'a3
+
+            val fold_rec_weak :
+              (TE.key -> 'a1 -> 'a2 -> 'a2) -> 'a2 -> ('a1 TE.t -> 'a1 TE.t
+              -> 'a2 -> __ -> 'a3 -> 'a3) -> 'a3 -> (TE.key -> 'a1 -> 'a2 ->
+              'a1 TE.t -> __ -> 'a3 -> 'a3) -> 'a1 TE.t -> 'a3
+
+            val fold_rel :
+              (TE.key -> 'a1 -> 'a2 -> 'a2) -> (TE.key -> 'a1 -> 'a3 -> 'a3)
+              -> 'a2 -> 'a3 -> 'a1 TE.t -> 'a4 -> (TE.key -> 'a1 -> 'a2 ->
+              'a3 -> __ -> 'a4 -> 'a4) -> 'a4
+
+            val map_induction :
+              ('a1 TE.t -> __ -> 'a2) -> ('a1 TE.t -> 'a1 TE.t -> 'a2 ->
+              TE.key -> 'a1 -> __ -> __ -> 'a2) -> 'a1 TE.t -> 'a2
+
+            val map_induction_bis :
+              ('a1 TE.t -> 'a1 TE.t -> __ -> 'a2 -> 'a2) -> 'a2 -> (TE.key ->
+              'a1 -> 'a1 TE.t -> __ -> 'a2 -> 'a2) -> 'a1 TE.t -> 'a2
+
+            val cardinal_inv_2 : 'a1 TE.t -> int -> (TE.key * 'a1)
+
+            val cardinal_inv_2b : 'a1 TE.t -> (TE.key * 'a1)
+
+            val filter : (TE.key -> 'a1 -> bool) -> 'a1 TE.t -> 'a1 TE.t
+
+            val for_all : (TE.key -> 'a1 -> bool) -> 'a1 TE.t -> bool
+
+            val exists_ : (TE.key -> 'a1 -> bool) -> 'a1 TE.t -> bool
+
+            val partition :
+              (TE.key -> 'a1 -> bool) -> 'a1 TE.t -> 'a1 TE.t * 'a1 TE.t
+
+            val update : 'a1 TE.t -> 'a1 TE.t -> 'a1 TE.t
+
+            val restrict : 'a1 TE.t -> 'a1 TE.t -> 'a1 TE.t
+
+            val diff : 'a1 TE.t -> 'a1 TE.t -> 'a1 TE.t
+
+            val coq_Partition_In :
+              'a1 TE.t -> 'a1 TE.t -> 'a1 TE.t -> TE.key -> bool
+
+            val update_dec : 'a1 TE.t -> 'a1 TE.t -> TE.key -> 'a1 -> bool
+
+            val filter_dom : (TE.key -> bool) -> 'a1 TE.t -> 'a1 TE.t
+
+            val filter_range : ('a1 -> bool) -> 'a1 TE.t -> 'a1 TE.t
+
+            val for_all_dom : (TE.key -> bool) -> 'a1 TE.t -> bool
+
+            val for_all_range : ('a1 -> bool) -> 'a1 TE.t -> bool
+
+            val exists_dom : (TE.key -> bool) -> 'a1 TE.t -> bool
+
+            val exists_range : ('a1 -> bool) -> 'a1 TE.t -> bool
+
+            val partition_dom :
+              (TE.key -> bool) -> 'a1 TE.t -> 'a1 TE.t * 'a1 TE.t
+
+            val partition_range :
+              ('a1 -> bool) -> 'a1 TE.t -> 'a1 TE.t * 'a1 TE.t
+           end
+
+          val gtb : (TE.key * 'a1) -> (TE.key * 'a1) -> bool
+
+          val leb : (TE.key * 'a1) -> (TE.key * 'a1) -> bool
+
+          val elements_lt : (TE.key * 'a1) -> 'a1 TE.t -> (TE.key * 'a1) list
+
+          val elements_ge : (TE.key * 'a1) -> 'a1 TE.t -> (TE.key * 'a1) list
+
+          val max_elt_aux : (TE.key * 'a1) list -> (TE.key * 'a1) option
+
+          val max_elt : 'a1 TE.t -> (TE.key * 'a1) option
+
+          val min_elt : 'a1 TE.t -> (TE.key * 'a1) option
+
+          val map_induction_max :
+            ('a1 TE.t -> __ -> 'a2) -> ('a1 TE.t -> 'a1 TE.t -> 'a2 ->
+            Equality.sort -> 'a1 -> __ -> __ -> 'a2) -> 'a1 TE.t -> 'a2
+
+          val map_induction_min :
+            ('a1 TE.t -> __ -> 'a2) -> ('a1 TE.t -> 'a1 TE.t -> 'a2 ->
+            Equality.sort -> 'a1 -> __ -> __ -> 'a2) -> 'a1 TE.t -> 'a2
+         end
+
+        val eqb : Equality.sort -> Equality.sort -> bool
+
+        val coq_In_dec : 'a1 TE.t -> TE.key -> bool
+
+        module ME :
+         sig
+          module TO :
+           sig
+            type t = Equality.sort
+           end
+
+          module IsTO :
+           sig
+           end
+
+          module OrderTac :
+           sig
+           end
+
+          val eq_dec : Equality.sort -> Equality.sort -> bool
+
+          val lt_dec : Equality.sort -> Equality.sort -> bool
+
+          val eqb : Equality.sort -> Equality.sort -> bool
+         end
+
+        module O :
+         sig
+          module MO :
+           sig
+            module TO :
+             sig
+              type t = Equality.sort
+             end
+
+            module IsTO :
+             sig
+             end
+
+            module OrderTac :
+             sig
+             end
+
+            val eq_dec : Equality.sort -> Equality.sort -> bool
+
+            val lt_dec : Equality.sort -> Equality.sort -> bool
+
+            val eqb : Equality.sort -> Equality.sort -> bool
+           end
+         end
+
+        module P :
+         sig
+          module F :
+           sig
+            val eqb : Equality.sort -> Equality.sort -> bool
+
+            val coq_In_dec : 'a1 TE.t -> TE.key -> bool
+           end
+
+          val uncurry : ('a1 -> 'a2 -> 'a3) -> ('a1 * 'a2) -> 'a3
+
+          val of_list : (TE.key * 'a1) list -> 'a1 TE.t
+
+          val to_list : 'a1 TE.t -> (TE.key * 'a1) list
+
+          val fold_rec :
+            (TE.key -> 'a1 -> 'a2 -> 'a2) -> 'a2 -> 'a1 TE.t -> ('a1 TE.t ->
+            __ -> 'a3) -> (TE.key -> 'a1 -> 'a2 -> 'a1 TE.t -> 'a1 TE.t -> __
+            -> __ -> __ -> 'a3 -> 'a3) -> 'a3
+
+          val fold_rec_bis :
+            (TE.key -> 'a1 -> 'a2 -> 'a2) -> 'a2 -> 'a1 TE.t -> ('a1 TE.t ->
+            'a1 TE.t -> 'a2 -> __ -> 'a3 -> 'a3) -> 'a3 -> (TE.key -> 'a1 ->
+            'a2 -> 'a1 TE.t -> __ -> __ -> 'a3 -> 'a3) -> 'a3
+
+          val fold_rec_nodep :
+            (TE.key -> 'a1 -> 'a2 -> 'a2) -> 'a2 -> 'a1 TE.t -> 'a3 ->
+            (TE.key -> 'a1 -> 'a2 -> __ -> 'a3 -> 'a3) -> 'a3
+
+          val fold_rec_weak :
+            (TE.key -> 'a1 -> 'a2 -> 'a2) -> 'a2 -> ('a1 TE.t -> 'a1 TE.t ->
+            'a2 -> __ -> 'a3 -> 'a3) -> 'a3 -> (TE.key -> 'a1 -> 'a2 -> 'a1
+            TE.t -> __ -> 'a3 -> 'a3) -> 'a1 TE.t -> 'a3
+
+          val fold_rel :
+            (TE.key -> 'a1 -> 'a2 -> 'a2) -> (TE.key -> 'a1 -> 'a3 -> 'a3) ->
+            'a2 -> 'a3 -> 'a1 TE.t -> 'a4 -> (TE.key -> 'a1 -> 'a2 -> 'a3 ->
+            __ -> 'a4 -> 'a4) -> 'a4
+
+          val map_induction :
+            ('a1 TE.t -> __ -> 'a2) -> ('a1 TE.t -> 'a1 TE.t -> 'a2 -> TE.key
+            -> 'a1 -> __ -> __ -> 'a2) -> 'a1 TE.t -> 'a2
+
+          val map_induction_bis :
+            ('a1 TE.t -> 'a1 TE.t -> __ -> 'a2 -> 'a2) -> 'a2 -> (TE.key ->
+            'a1 -> 'a1 TE.t -> __ -> 'a2 -> 'a2) -> 'a1 TE.t -> 'a2
+
+          val cardinal_inv_2 : 'a1 TE.t -> int -> (TE.key * 'a1)
+
+          val cardinal_inv_2b : 'a1 TE.t -> (TE.key * 'a1)
+
+          val filter : (TE.key -> 'a1 -> bool) -> 'a1 TE.t -> 'a1 TE.t
+
+          val for_all : (TE.key -> 'a1 -> bool) -> 'a1 TE.t -> bool
+
+          val exists_ : (TE.key -> 'a1 -> bool) -> 'a1 TE.t -> bool
+
+          val partition :
+            (TE.key -> 'a1 -> bool) -> 'a1 TE.t -> 'a1 TE.t * 'a1 TE.t
+
+          val update : 'a1 TE.t -> 'a1 TE.t -> 'a1 TE.t
+
+          val restrict : 'a1 TE.t -> 'a1 TE.t -> 'a1 TE.t
+
+          val diff : 'a1 TE.t -> 'a1 TE.t -> 'a1 TE.t
+
+          val coq_Partition_In :
+            'a1 TE.t -> 'a1 TE.t -> 'a1 TE.t -> TE.key -> bool
+
+          val update_dec : 'a1 TE.t -> 'a1 TE.t -> TE.key -> 'a1 -> bool
+
+          val filter_dom : (TE.key -> bool) -> 'a1 TE.t -> 'a1 TE.t
+
+          val filter_range : ('a1 -> bool) -> 'a1 TE.t -> 'a1 TE.t
+
+          val for_all_dom : (TE.key -> bool) -> 'a1 TE.t -> bool
+
+          val for_all_range : ('a1 -> bool) -> 'a1 TE.t -> bool
+
+          val exists_dom : (TE.key -> bool) -> 'a1 TE.t -> bool
+
+          val exists_range : ('a1 -> bool) -> 'a1 TE.t -> bool
+
+          val partition_dom :
+            (TE.key -> bool) -> 'a1 TE.t -> 'a1 TE.t * 'a1 TE.t
+
+          val partition_range :
+            ('a1 -> bool) -> 'a1 TE.t -> 'a1 TE.t * 'a1 TE.t
+         end
+
+        val gtb : (TE.key * 'a1) -> (TE.key * 'a1) -> bool
+
+        val leb : (TE.key * 'a1) -> (TE.key * 'a1) -> bool
+
+        val elements_lt : (TE.key * 'a1) -> 'a1 TE.t -> (TE.key * 'a1) list
+
+        val elements_ge : (TE.key * 'a1) -> 'a1 TE.t -> (TE.key * 'a1) list
+
+        val max_elt_aux : (TE.key * 'a1) list -> (TE.key * 'a1) option
+
+        val max_elt : 'a1 TE.t -> (TE.key * 'a1) option
+
+        val min_elt : 'a1 TE.t -> (TE.key * 'a1) option
+
+        val map_induction_max :
+          ('a1 TE.t -> __ -> 'a2) -> ('a1 TE.t -> 'a1 TE.t -> 'a2 ->
+          Equality.sort -> 'a1 -> __ -> __ -> 'a2) -> 'a1 TE.t -> 'a2
+
+        val map_induction_min :
+          ('a1 TE.t -> __ -> 'a2) -> ('a1 TE.t -> 'a1 TE.t -> 'a2 ->
+          Equality.sort -> 'a1 -> __ -> __ -> 'a2) -> 'a1 TE.t -> 'a2
+
+        val memP : TE.key -> 'a1 TE.t -> reflect
+
+        val split : ('a1 * 'a2) TE.t -> 'a1 TE.t * 'a2 TE.t
+
+        module EFacts :
+         sig
+          module TO :
+           sig
+            type t = Equality.sort
+           end
+
+          module IsTO :
+           sig
+           end
+
+          module OrderTac :
+           sig
+           end
+
+          val eq_dec : Equality.sort -> Equality.sort -> bool
+
+          val lt_dec : Equality.sort -> Equality.sort -> bool
+
+          val eqb : Equality.sort -> Equality.sort -> bool
+         end
+
+        val max_opt : TE.key -> TE.key option -> TE.key
+
+        val max_key_elements : (TE.key * 'a1) list -> TE.key option
+
+        val max_key : 'a1 TE.t -> TE.key option
+
+        val min_opt : TE.key -> TE.key option -> TE.key
+
+        val min_key_elements : (TE.key * 'a1) list -> TE.key option
+
+        val min_key : 'a1 TE.t -> TE.key option
+       end
+     end
+
+    module VSLemmas :
+     sig
+      module F :
+       sig
+        val eqb : Equality.sort -> Equality.sort -> bool
+       end
+
+      module OP :
+       sig
+        module ME :
+         sig
+          module TO :
+           sig
+            type t = Equality.sort
+           end
+
+          module IsTO :
+           sig
+           end
+
+          module OrderTac :
+           sig
+           end
+
+          val eq_dec : Equality.sort -> Equality.sort -> bool
+
+          val lt_dec : Equality.sort -> Equality.sort -> bool
+
+          val eqb : Equality.sort -> Equality.sort -> bool
+         end
+
+        module P :
+         sig
+          module Dec :
+           sig
+            module F :
+             sig
+              val eqb : Equality.sort -> Equality.sort -> bool
+             end
+
+            module FSetLogicalFacts :
+             sig
+             end
+
+            module FSetDecideAuxiliary :
+             sig
+             end
+
+            module FSetDecideTestCases :
+             sig
+             end
+           end
+
+          module FM :
+           sig
+            val eqb : Equality.sort -> Equality.sort -> bool
+           end
+
+          val coq_In_dec : VS.elt -> VS.t -> bool
+
+          val of_list : VS.elt list -> VS.t
+
+          val to_list : VS.t -> VS.elt list
+
+          val fold_rec :
+            (VS.elt -> 'a1 -> 'a1) -> 'a1 -> VS.t -> (VS.t -> __ -> 'a2) ->
+            (VS.elt -> 'a1 -> VS.t -> VS.t -> __ -> __ -> __ -> 'a2 -> 'a2)
+            -> 'a2
+
+          val fold_rec_bis :
+            (VS.elt -> 'a1 -> 'a1) -> 'a1 -> VS.t -> (VS.t -> VS.t -> 'a1 ->
+            __ -> 'a2 -> 'a2) -> 'a2 -> (VS.elt -> 'a1 -> VS.t -> __ -> __ ->
+            'a2 -> 'a2) -> 'a2
+
+          val fold_rec_nodep :
+            (VS.elt -> 'a1 -> 'a1) -> 'a1 -> VS.t -> 'a2 -> (VS.elt -> 'a1 ->
+            __ -> 'a2 -> 'a2) -> 'a2
+
+          val fold_rec_weak :
+            (VS.elt -> 'a1 -> 'a1) -> 'a1 -> (VS.t -> VS.t -> 'a1 -> __ ->
+            'a2 -> 'a2) -> 'a2 -> (VS.elt -> 'a1 -> VS.t -> __ -> 'a2 -> 'a2)
+            -> VS.t -> 'a2
+
+          val fold_rel :
+            (VS.elt -> 'a1 -> 'a1) -> (VS.elt -> 'a2 -> 'a2) -> 'a1 -> 'a2 ->
+            VS.t -> 'a3 -> (VS.elt -> 'a1 -> 'a2 -> __ -> 'a3 -> 'a3) -> 'a3
+
+          val set_induction :
+            (VS.t -> __ -> 'a1) -> (VS.t -> VS.t -> 'a1 -> VS.elt -> __ -> __
+            -> 'a1) -> VS.t -> 'a1
+
+          val set_induction_bis :
+            (VS.t -> VS.t -> __ -> 'a1 -> 'a1) -> 'a1 -> (VS.elt -> VS.t ->
+            __ -> 'a1 -> 'a1) -> VS.t -> 'a1
+
+          val cardinal_inv_2 : VS.t -> int -> VS.elt
+
+          val cardinal_inv_2b : VS.t -> VS.elt
+         end
+
+        val gtb : Equality.sort -> Equality.sort -> bool
+
+        val leb : Equality.sort -> Equality.sort -> bool
+
+        val elements_lt : Equality.sort -> VS.t -> Equality.sort list
+
+        val elements_ge : Equality.sort -> VS.t -> Equality.sort list
+
+        val set_induction_max :
+          (VS.t -> __ -> 'a1) -> (VS.t -> VS.t -> 'a1 -> Equality.sort -> __
+          -> __ -> 'a1) -> VS.t -> 'a1
+
+        val set_induction_min :
+          (VS.t -> __ -> 'a1) -> (VS.t -> VS.t -> 'a1 -> Equality.sort -> __
+          -> __ -> 'a1) -> VS.t -> 'a1
+       end
+
+      val eqb : Equality.sort -> Equality.sort -> bool
+
+      module ME :
+       sig
+        module TO :
+         sig
+          type t = Equality.sort
+         end
+
+        module IsTO :
+         sig
+         end
+
+        module OrderTac :
+         sig
+         end
+
+        val eq_dec : Equality.sort -> Equality.sort -> bool
+
+        val lt_dec : Equality.sort -> Equality.sort -> bool
+
+        val eqb : Equality.sort -> Equality.sort -> bool
+       end
+
+      module P :
+       sig
+        module Dec :
+         sig
+          module F :
+           sig
+            val eqb : Equality.sort -> Equality.sort -> bool
+           end
+
+          module FSetLogicalFacts :
+           sig
+           end
+
+          module FSetDecideAuxiliary :
+           sig
+           end
+
+          module FSetDecideTestCases :
+           sig
+           end
+         end
+
+        module FM :
+         sig
+          val eqb : Equality.sort -> Equality.sort -> bool
+         end
+
+        val coq_In_dec : VS.elt -> VS.t -> bool
+
+        val of_list : VS.elt list -> VS.t
+
+        val to_list : VS.t -> VS.elt list
+
+        val fold_rec :
+          (VS.elt -> 'a1 -> 'a1) -> 'a1 -> VS.t -> (VS.t -> __ -> 'a2) ->
+          (VS.elt -> 'a1 -> VS.t -> VS.t -> __ -> __ -> __ -> 'a2 -> 'a2) ->
+          'a2
+
+        val fold_rec_bis :
+          (VS.elt -> 'a1 -> 'a1) -> 'a1 -> VS.t -> (VS.t -> VS.t -> 'a1 -> __
+          -> 'a2 -> 'a2) -> 'a2 -> (VS.elt -> 'a1 -> VS.t -> __ -> __ -> 'a2
+          -> 'a2) -> 'a2
+
+        val fold_rec_nodep :
+          (VS.elt -> 'a1 -> 'a1) -> 'a1 -> VS.t -> 'a2 -> (VS.elt -> 'a1 ->
+          __ -> 'a2 -> 'a2) -> 'a2
+
+        val fold_rec_weak :
+          (VS.elt -> 'a1 -> 'a1) -> 'a1 -> (VS.t -> VS.t -> 'a1 -> __ -> 'a2
+          -> 'a2) -> 'a2 -> (VS.elt -> 'a1 -> VS.t -> __ -> 'a2 -> 'a2) ->
+          VS.t -> 'a2
+
+        val fold_rel :
+          (VS.elt -> 'a1 -> 'a1) -> (VS.elt -> 'a2 -> 'a2) -> 'a1 -> 'a2 ->
+          VS.t -> 'a3 -> (VS.elt -> 'a1 -> 'a2 -> __ -> 'a3 -> 'a3) -> 'a3
+
+        val set_induction :
+          (VS.t -> __ -> 'a1) -> (VS.t -> VS.t -> 'a1 -> VS.elt -> __ -> __
+          -> 'a1) -> VS.t -> 'a1
+
+        val set_induction_bis :
+          (VS.t -> VS.t -> __ -> 'a1 -> 'a1) -> 'a1 -> (VS.elt -> VS.t -> __
+          -> 'a1 -> 'a1) -> VS.t -> 'a1
+
+        val cardinal_inv_2 : VS.t -> int -> VS.elt
+
+        val cardinal_inv_2b : VS.t -> VS.elt
+       end
+
+      val gtb : Equality.sort -> Equality.sort -> bool
+
+      val leb : Equality.sort -> Equality.sort -> bool
+
+      val elements_lt : Equality.sort -> VS.t -> Equality.sort list
+
+      val elements_ge : Equality.sort -> VS.t -> Equality.sort list
+
+      val set_induction_max :
+        (VS.t -> __ -> 'a1) -> (VS.t -> VS.t -> 'a1 -> Equality.sort -> __ ->
+        __ -> 'a1) -> VS.t -> 'a1
+
+      val set_induction_min :
+        (VS.t -> __ -> 'a1) -> (VS.t -> VS.t -> 'a1 -> Equality.sort -> __ ->
+        __ -> 'a1) -> VS.t -> 'a1
+
+      val memP : VS.elt -> VS.t -> reflect
+
+      val equalP : VS.t -> VS.t -> reflect
+
+      val subsetP : VS.t -> VS.t -> reflect
+
+      val emptyP : VS.t -> reflect
+
+      val disjoint : VS.t -> VS.t -> bool
+
+      val proper_subset : VS.t -> VS.t -> bool
+     end
+
+    module VMLemmas :
+     sig
+      module F :
+       sig
+        val eqb : Equality.sort -> Equality.sort -> bool
+
+        val coq_In_dec : 'a1 TE.t -> TE.key -> bool
+       end
+
+      module OP :
+       sig
+        module ME :
+         sig
+          module TO :
+           sig
+            type t = Equality.sort
+           end
+
+          module IsTO :
+           sig
+           end
+
+          module OrderTac :
+           sig
+           end
+
+          val eq_dec : Equality.sort -> Equality.sort -> bool
+
+          val lt_dec : Equality.sort -> Equality.sort -> bool
+
+          val eqb : Equality.sort -> Equality.sort -> bool
+         end
+
+        module O :
+         sig
+          module MO :
+           sig
+            module TO :
+             sig
+              type t = Equality.sort
+             end
+
+            module IsTO :
+             sig
+             end
+
+            module OrderTac :
+             sig
+             end
+
+            val eq_dec : Equality.sort -> Equality.sort -> bool
+
+            val lt_dec : Equality.sort -> Equality.sort -> bool
+
+            val eqb : Equality.sort -> Equality.sort -> bool
+           end
+         end
+
+        module P :
+         sig
+          module F :
+           sig
+            val eqb : Equality.sort -> Equality.sort -> bool
+
+            val coq_In_dec : 'a1 TE.t -> TE.key -> bool
+           end
+
+          val uncurry : ('a1 -> 'a2 -> 'a3) -> ('a1 * 'a2) -> 'a3
+
+          val of_list : (TE.key * 'a1) list -> 'a1 TE.t
+
+          val to_list : 'a1 TE.t -> (TE.key * 'a1) list
+
+          val fold_rec :
+            (TE.key -> 'a1 -> 'a2 -> 'a2) -> 'a2 -> 'a1 TE.t -> ('a1 TE.t ->
+            __ -> 'a3) -> (TE.key -> 'a1 -> 'a2 -> 'a1 TE.t -> 'a1 TE.t -> __
+            -> __ -> __ -> 'a3 -> 'a3) -> 'a3
+
+          val fold_rec_bis :
+            (TE.key -> 'a1 -> 'a2 -> 'a2) -> 'a2 -> 'a1 TE.t -> ('a1 TE.t ->
+            'a1 TE.t -> 'a2 -> __ -> 'a3 -> 'a3) -> 'a3 -> (TE.key -> 'a1 ->
+            'a2 -> 'a1 TE.t -> __ -> __ -> 'a3 -> 'a3) -> 'a3
+
+          val fold_rec_nodep :
+            (TE.key -> 'a1 -> 'a2 -> 'a2) -> 'a2 -> 'a1 TE.t -> 'a3 ->
+            (TE.key -> 'a1 -> 'a2 -> __ -> 'a3 -> 'a3) -> 'a3
+
+          val fold_rec_weak :
+            (TE.key -> 'a1 -> 'a2 -> 'a2) -> 'a2 -> ('a1 TE.t -> 'a1 TE.t ->
+            'a2 -> __ -> 'a3 -> 'a3) -> 'a3 -> (TE.key -> 'a1 -> 'a2 -> 'a1
+            TE.t -> __ -> 'a3 -> 'a3) -> 'a1 TE.t -> 'a3
+
+          val fold_rel :
+            (TE.key -> 'a1 -> 'a2 -> 'a2) -> (TE.key -> 'a1 -> 'a3 -> 'a3) ->
+            'a2 -> 'a3 -> 'a1 TE.t -> 'a4 -> (TE.key -> 'a1 -> 'a2 -> 'a3 ->
+            __ -> 'a4 -> 'a4) -> 'a4
+
+          val map_induction :
+            ('a1 TE.t -> __ -> 'a2) -> ('a1 TE.t -> 'a1 TE.t -> 'a2 -> TE.key
+            -> 'a1 -> __ -> __ -> 'a2) -> 'a1 TE.t -> 'a2
+
+          val map_induction_bis :
+            ('a1 TE.t -> 'a1 TE.t -> __ -> 'a2 -> 'a2) -> 'a2 -> (TE.key ->
+            'a1 -> 'a1 TE.t -> __ -> 'a2 -> 'a2) -> 'a1 TE.t -> 'a2
+
+          val cardinal_inv_2 : 'a1 TE.t -> int -> (TE.key * 'a1)
+
+          val cardinal_inv_2b : 'a1 TE.t -> (TE.key * 'a1)
+
+          val filter : (TE.key -> 'a1 -> bool) -> 'a1 TE.t -> 'a1 TE.t
+
+          val for_all : (TE.key -> 'a1 -> bool) -> 'a1 TE.t -> bool
+
+          val exists_ : (TE.key -> 'a1 -> bool) -> 'a1 TE.t -> bool
+
+          val partition :
+            (TE.key -> 'a1 -> bool) -> 'a1 TE.t -> 'a1 TE.t * 'a1 TE.t
+
+          val update : 'a1 TE.t -> 'a1 TE.t -> 'a1 TE.t
+
+          val restrict : 'a1 TE.t -> 'a1 TE.t -> 'a1 TE.t
+
+          val diff : 'a1 TE.t -> 'a1 TE.t -> 'a1 TE.t
+
+          val coq_Partition_In :
+            'a1 TE.t -> 'a1 TE.t -> 'a1 TE.t -> TE.key -> bool
+
+          val update_dec : 'a1 TE.t -> 'a1 TE.t -> TE.key -> 'a1 -> bool
+
+          val filter_dom : (TE.key -> bool) -> 'a1 TE.t -> 'a1 TE.t
+
+          val filter_range : ('a1 -> bool) -> 'a1 TE.t -> 'a1 TE.t
+
+          val for_all_dom : (TE.key -> bool) -> 'a1 TE.t -> bool
+
+          val for_all_range : ('a1 -> bool) -> 'a1 TE.t -> bool
+
+          val exists_dom : (TE.key -> bool) -> 'a1 TE.t -> bool
+
+          val exists_range : ('a1 -> bool) -> 'a1 TE.t -> bool
+
+          val partition_dom :
+            (TE.key -> bool) -> 'a1 TE.t -> 'a1 TE.t * 'a1 TE.t
+
+          val partition_range :
+            ('a1 -> bool) -> 'a1 TE.t -> 'a1 TE.t * 'a1 TE.t
+         end
+
+        val gtb : (TE.key * 'a1) -> (TE.key * 'a1) -> bool
+
+        val leb : (TE.key * 'a1) -> (TE.key * 'a1) -> bool
+
+        val elements_lt : (TE.key * 'a1) -> 'a1 TE.t -> (TE.key * 'a1) list
+
+        val elements_ge : (TE.key * 'a1) -> 'a1 TE.t -> (TE.key * 'a1) list
+
+        val max_elt_aux : (TE.key * 'a1) list -> (TE.key * 'a1) option
+
+        val max_elt : 'a1 TE.t -> (TE.key * 'a1) option
+
+        val min_elt : 'a1 TE.t -> (TE.key * 'a1) option
+
+        val map_induction_max :
+          ('a1 TE.t -> __ -> 'a2) -> ('a1 TE.t -> 'a1 TE.t -> 'a2 ->
+          Equality.sort -> 'a1 -> __ -> __ -> 'a2) -> 'a1 TE.t -> 'a2
+
+        val map_induction_min :
+          ('a1 TE.t -> __ -> 'a2) -> ('a1 TE.t -> 'a1 TE.t -> 'a2 ->
+          Equality.sort -> 'a1 -> __ -> __ -> 'a2) -> 'a1 TE.t -> 'a2
+       end
+
+      val eqb : Equality.sort -> Equality.sort -> bool
+
+      val coq_In_dec : 'a1 TE.t -> TE.key -> bool
+
+      module ME :
+       sig
+        module TO :
+         sig
+          type t = Equality.sort
+         end
+
+        module IsTO :
+         sig
+         end
+
+        module OrderTac :
+         sig
+         end
+
+        val eq_dec : Equality.sort -> Equality.sort -> bool
+
+        val lt_dec : Equality.sort -> Equality.sort -> bool
+
+        val eqb : Equality.sort -> Equality.sort -> bool
+       end
+
+      module O :
+       sig
+        module MO :
+         sig
+          module TO :
+           sig
+            type t = Equality.sort
+           end
+
+          module IsTO :
+           sig
+           end
+
+          module OrderTac :
+           sig
+           end
+
+          val eq_dec : Equality.sort -> Equality.sort -> bool
+
+          val lt_dec : Equality.sort -> Equality.sort -> bool
+
+          val eqb : Equality.sort -> Equality.sort -> bool
+         end
+       end
+
+      module P :
+       sig
+        module F :
+         sig
+          val eqb : Equality.sort -> Equality.sort -> bool
+
+          val coq_In_dec : 'a1 TE.t -> TE.key -> bool
+         end
+
+        val uncurry : ('a1 -> 'a2 -> 'a3) -> ('a1 * 'a2) -> 'a3
+
+        val of_list : (TE.key * 'a1) list -> 'a1 TE.t
+
+        val to_list : 'a1 TE.t -> (TE.key * 'a1) list
+
+        val fold_rec :
+          (TE.key -> 'a1 -> 'a2 -> 'a2) -> 'a2 -> 'a1 TE.t -> ('a1 TE.t -> __
+          -> 'a3) -> (TE.key -> 'a1 -> 'a2 -> 'a1 TE.t -> 'a1 TE.t -> __ ->
+          __ -> __ -> 'a3 -> 'a3) -> 'a3
+
+        val fold_rec_bis :
+          (TE.key -> 'a1 -> 'a2 -> 'a2) -> 'a2 -> 'a1 TE.t -> ('a1 TE.t ->
+          'a1 TE.t -> 'a2 -> __ -> 'a3 -> 'a3) -> 'a3 -> (TE.key -> 'a1 ->
+          'a2 -> 'a1 TE.t -> __ -> __ -> 'a3 -> 'a3) -> 'a3
+
+        val fold_rec_nodep :
+          (TE.key -> 'a1 -> 'a2 -> 'a2) -> 'a2 -> 'a1 TE.t -> 'a3 -> (TE.key
+          -> 'a1 -> 'a2 -> __ -> 'a3 -> 'a3) -> 'a3
+
+        val fold_rec_weak :
+          (TE.key -> 'a1 -> 'a2 -> 'a2) -> 'a2 -> ('a1 TE.t -> 'a1 TE.t ->
+          'a2 -> __ -> 'a3 -> 'a3) -> 'a3 -> (TE.key -> 'a1 -> 'a2 -> 'a1
+          TE.t -> __ -> 'a3 -> 'a3) -> 'a1 TE.t -> 'a3
+
+        val fold_rel :
+          (TE.key -> 'a1 -> 'a2 -> 'a2) -> (TE.key -> 'a1 -> 'a3 -> 'a3) ->
+          'a2 -> 'a3 -> 'a1 TE.t -> 'a4 -> (TE.key -> 'a1 -> 'a2 -> 'a3 -> __
+          -> 'a4 -> 'a4) -> 'a4
+
+        val map_induction :
+          ('a1 TE.t -> __ -> 'a2) -> ('a1 TE.t -> 'a1 TE.t -> 'a2 -> TE.key
+          -> 'a1 -> __ -> __ -> 'a2) -> 'a1 TE.t -> 'a2
+
+        val map_induction_bis :
+          ('a1 TE.t -> 'a1 TE.t -> __ -> 'a2 -> 'a2) -> 'a2 -> (TE.key -> 'a1
+          -> 'a1 TE.t -> __ -> 'a2 -> 'a2) -> 'a1 TE.t -> 'a2
+
+        val cardinal_inv_2 : 'a1 TE.t -> int -> (TE.key * 'a1)
+
+        val cardinal_inv_2b : 'a1 TE.t -> (TE.key * 'a1)
+
+        val filter : (TE.key -> 'a1 -> bool) -> 'a1 TE.t -> 'a1 TE.t
+
+        val for_all : (TE.key -> 'a1 -> bool) -> 'a1 TE.t -> bool
+
+        val exists_ : (TE.key -> 'a1 -> bool) -> 'a1 TE.t -> bool
+
+        val partition :
+          (TE.key -> 'a1 -> bool) -> 'a1 TE.t -> 'a1 TE.t * 'a1 TE.t
+
+        val update : 'a1 TE.t -> 'a1 TE.t -> 'a1 TE.t
+
+        val restrict : 'a1 TE.t -> 'a1 TE.t -> 'a1 TE.t
+
+        val diff : 'a1 TE.t -> 'a1 TE.t -> 'a1 TE.t
+
+        val coq_Partition_In :
+          'a1 TE.t -> 'a1 TE.t -> 'a1 TE.t -> TE.key -> bool
+
+        val update_dec : 'a1 TE.t -> 'a1 TE.t -> TE.key -> 'a1 -> bool
+
+        val filter_dom : (TE.key -> bool) -> 'a1 TE.t -> 'a1 TE.t
+
+        val filter_range : ('a1 -> bool) -> 'a1 TE.t -> 'a1 TE.t
+
+        val for_all_dom : (TE.key -> bool) -> 'a1 TE.t -> bool
+
+        val for_all_range : ('a1 -> bool) -> 'a1 TE.t -> bool
+
+        val exists_dom : (TE.key -> bool) -> 'a1 TE.t -> bool
+
+        val exists_range : ('a1 -> bool) -> 'a1 TE.t -> bool
+
+        val partition_dom :
+          (TE.key -> bool) -> 'a1 TE.t -> 'a1 TE.t * 'a1 TE.t
+
+        val partition_range : ('a1 -> bool) -> 'a1 TE.t -> 'a1 TE.t * 'a1 TE.t
+       end
+
+      val gtb : (TE.key * 'a1) -> (TE.key * 'a1) -> bool
+
+      val leb : (TE.key * 'a1) -> (TE.key * 'a1) -> bool
+
+      val elements_lt : (TE.key * 'a1) -> 'a1 TE.t -> (TE.key * 'a1) list
+
+      val elements_ge : (TE.key * 'a1) -> 'a1 TE.t -> (TE.key * 'a1) list
+
+      val max_elt_aux : (TE.key * 'a1) list -> (TE.key * 'a1) option
+
+      val max_elt : 'a1 TE.t -> (TE.key * 'a1) option
+
+      val min_elt : 'a1 TE.t -> (TE.key * 'a1) option
+
+      val map_induction_max :
+        ('a1 TE.t -> __ -> 'a2) -> ('a1 TE.t -> 'a1 TE.t -> 'a2 ->
+        Equality.sort -> 'a1 -> __ -> __ -> 'a2) -> 'a1 TE.t -> 'a2
+
+      val map_induction_min :
+        ('a1 TE.t -> __ -> 'a2) -> ('a1 TE.t -> 'a1 TE.t -> 'a2 ->
+        Equality.sort -> 'a1 -> __ -> __ -> 'a2) -> 'a1 TE.t -> 'a2
+
+      val memP : TE.key -> 'a1 TE.t -> reflect
+
+      val split : ('a1 * 'a2) TE.t -> 'a1 TE.t * 'a2 TE.t
+
+      module EFacts :
+       sig
+        module TO :
+         sig
+          type t = Equality.sort
+         end
+
+        module IsTO :
+         sig
+         end
+
+        module OrderTac :
+         sig
+         end
+
+        val eq_dec : Equality.sort -> Equality.sort -> bool
+
+        val lt_dec : Equality.sort -> Equality.sort -> bool
+
+        val eqb : Equality.sort -> Equality.sort -> bool
+       end
+
+      val max_opt : TE.key -> TE.key option -> TE.key
+
+      val max_key_elements : (TE.key * 'a1) list -> TE.key option
+
+      val max_key : 'a1 TE.t -> TE.key option
+
+      val min_opt : TE.key -> TE.key option -> TE.key
+
+      val min_key_elements : (TE.key * 'a1) list -> TE.key option
+
+      val min_key : 'a1 TE.t -> TE.key option
+     end
+   end
  end
 
 module QFBV :
@@ -2467,6 +3697,1383 @@ module QFBV :
   val string_of_exp : exp -> char list
 
   val string_of_bexp : bexp -> char list
+
+  module MA :
+   sig
+    module MA :
+     sig
+      module VSLemmas :
+       sig
+        module F :
+         sig
+          val eqb : Equality.sort -> Equality.sort -> bool
+         end
+
+        module OP :
+         sig
+          module ME :
+           sig
+            module TO :
+             sig
+              type t = Equality.sort
+             end
+
+            module IsTO :
+             sig
+             end
+
+            module OrderTac :
+             sig
+             end
+
+            val eq_dec : Equality.sort -> Equality.sort -> bool
+
+            val lt_dec : Equality.sort -> Equality.sort -> bool
+
+            val eqb : Equality.sort -> Equality.sort -> bool
+           end
+
+          module P :
+           sig
+            module Dec :
+             sig
+              module F :
+               sig
+                val eqb : Equality.sort -> Equality.sort -> bool
+               end
+
+              module FSetLogicalFacts :
+               sig
+               end
+
+              module FSetDecideAuxiliary :
+               sig
+               end
+
+              module FSetDecideTestCases :
+               sig
+               end
+             end
+
+            module FM :
+             sig
+              val eqb : Equality.sort -> Equality.sort -> bool
+             end
+
+            val coq_In_dec : SSAVS.elt -> SSAVS.t -> bool
+
+            val of_list : SSAVS.elt list -> SSAVS.t
+
+            val to_list : SSAVS.t -> SSAVS.elt list
+
+            val fold_rec :
+              (SSAVS.elt -> 'a1 -> 'a1) -> 'a1 -> SSAVS.t -> (SSAVS.t -> __
+              -> 'a2) -> (SSAVS.elt -> 'a1 -> SSAVS.t -> SSAVS.t -> __ -> __
+              -> __ -> 'a2 -> 'a2) -> 'a2
+
+            val fold_rec_bis :
+              (SSAVS.elt -> 'a1 -> 'a1) -> 'a1 -> SSAVS.t -> (SSAVS.t ->
+              SSAVS.t -> 'a1 -> __ -> 'a2 -> 'a2) -> 'a2 -> (SSAVS.elt -> 'a1
+              -> SSAVS.t -> __ -> __ -> 'a2 -> 'a2) -> 'a2
+
+            val fold_rec_nodep :
+              (SSAVS.elt -> 'a1 -> 'a1) -> 'a1 -> SSAVS.t -> 'a2 ->
+              (SSAVS.elt -> 'a1 -> __ -> 'a2 -> 'a2) -> 'a2
+
+            val fold_rec_weak :
+              (SSAVS.elt -> 'a1 -> 'a1) -> 'a1 -> (SSAVS.t -> SSAVS.t -> 'a1
+              -> __ -> 'a2 -> 'a2) -> 'a2 -> (SSAVS.elt -> 'a1 -> SSAVS.t ->
+              __ -> 'a2 -> 'a2) -> SSAVS.t -> 'a2
+
+            val fold_rel :
+              (SSAVS.elt -> 'a1 -> 'a1) -> (SSAVS.elt -> 'a2 -> 'a2) -> 'a1
+              -> 'a2 -> SSAVS.t -> 'a3 -> (SSAVS.elt -> 'a1 -> 'a2 -> __ ->
+              'a3 -> 'a3) -> 'a3
+
+            val set_induction :
+              (SSAVS.t -> __ -> 'a1) -> (SSAVS.t -> SSAVS.t -> 'a1 ->
+              SSAVS.elt -> __ -> __ -> 'a1) -> SSAVS.t -> 'a1
+
+            val set_induction_bis :
+              (SSAVS.t -> SSAVS.t -> __ -> 'a1 -> 'a1) -> 'a1 -> (SSAVS.elt
+              -> SSAVS.t -> __ -> 'a1 -> 'a1) -> SSAVS.t -> 'a1
+
+            val cardinal_inv_2 : SSAVS.t -> int -> SSAVS.elt
+
+            val cardinal_inv_2b : SSAVS.t -> SSAVS.elt
+           end
+
+          val gtb : Equality.sort -> Equality.sort -> bool
+
+          val leb : Equality.sort -> Equality.sort -> bool
+
+          val elements_lt : Equality.sort -> SSAVS.t -> Equality.sort list
+
+          val elements_ge : Equality.sort -> SSAVS.t -> Equality.sort list
+
+          val set_induction_max :
+            (SSAVS.t -> __ -> 'a1) -> (SSAVS.t -> SSAVS.t -> 'a1 ->
+            Equality.sort -> __ -> __ -> 'a1) -> SSAVS.t -> 'a1
+
+          val set_induction_min :
+            (SSAVS.t -> __ -> 'a1) -> (SSAVS.t -> SSAVS.t -> 'a1 ->
+            Equality.sort -> __ -> __ -> 'a1) -> SSAVS.t -> 'a1
+         end
+
+        val eqb : Equality.sort -> Equality.sort -> bool
+
+        module ME :
+         sig
+          module TO :
+           sig
+            type t = Equality.sort
+           end
+
+          module IsTO :
+           sig
+           end
+
+          module OrderTac :
+           sig
+           end
+
+          val eq_dec : Equality.sort -> Equality.sort -> bool
+
+          val lt_dec : Equality.sort -> Equality.sort -> bool
+
+          val eqb : Equality.sort -> Equality.sort -> bool
+         end
+
+        module P :
+         sig
+          module Dec :
+           sig
+            module F :
+             sig
+              val eqb : Equality.sort -> Equality.sort -> bool
+             end
+
+            module FSetLogicalFacts :
+             sig
+             end
+
+            module FSetDecideAuxiliary :
+             sig
+             end
+
+            module FSetDecideTestCases :
+             sig
+             end
+           end
+
+          module FM :
+           sig
+            val eqb : Equality.sort -> Equality.sort -> bool
+           end
+
+          val coq_In_dec : SSAVS.elt -> SSAVS.t -> bool
+
+          val of_list : SSAVS.elt list -> SSAVS.t
+
+          val to_list : SSAVS.t -> SSAVS.elt list
+
+          val fold_rec :
+            (SSAVS.elt -> 'a1 -> 'a1) -> 'a1 -> SSAVS.t -> (SSAVS.t -> __ ->
+            'a2) -> (SSAVS.elt -> 'a1 -> SSAVS.t -> SSAVS.t -> __ -> __ -> __
+            -> 'a2 -> 'a2) -> 'a2
+
+          val fold_rec_bis :
+            (SSAVS.elt -> 'a1 -> 'a1) -> 'a1 -> SSAVS.t -> (SSAVS.t ->
+            SSAVS.t -> 'a1 -> __ -> 'a2 -> 'a2) -> 'a2 -> (SSAVS.elt -> 'a1
+            -> SSAVS.t -> __ -> __ -> 'a2 -> 'a2) -> 'a2
+
+          val fold_rec_nodep :
+            (SSAVS.elt -> 'a1 -> 'a1) -> 'a1 -> SSAVS.t -> 'a2 -> (SSAVS.elt
+            -> 'a1 -> __ -> 'a2 -> 'a2) -> 'a2
+
+          val fold_rec_weak :
+            (SSAVS.elt -> 'a1 -> 'a1) -> 'a1 -> (SSAVS.t -> SSAVS.t -> 'a1 ->
+            __ -> 'a2 -> 'a2) -> 'a2 -> (SSAVS.elt -> 'a1 -> SSAVS.t -> __ ->
+            'a2 -> 'a2) -> SSAVS.t -> 'a2
+
+          val fold_rel :
+            (SSAVS.elt -> 'a1 -> 'a1) -> (SSAVS.elt -> 'a2 -> 'a2) -> 'a1 ->
+            'a2 -> SSAVS.t -> 'a3 -> (SSAVS.elt -> 'a1 -> 'a2 -> __ -> 'a3 ->
+            'a3) -> 'a3
+
+          val set_induction :
+            (SSAVS.t -> __ -> 'a1) -> (SSAVS.t -> SSAVS.t -> 'a1 -> SSAVS.elt
+            -> __ -> __ -> 'a1) -> SSAVS.t -> 'a1
+
+          val set_induction_bis :
+            (SSAVS.t -> SSAVS.t -> __ -> 'a1 -> 'a1) -> 'a1 -> (SSAVS.elt ->
+            SSAVS.t -> __ -> 'a1 -> 'a1) -> SSAVS.t -> 'a1
+
+          val cardinal_inv_2 : SSAVS.t -> int -> SSAVS.elt
+
+          val cardinal_inv_2b : SSAVS.t -> SSAVS.elt
+         end
+
+        val gtb : Equality.sort -> Equality.sort -> bool
+
+        val leb : Equality.sort -> Equality.sort -> bool
+
+        val elements_lt : Equality.sort -> SSAVS.t -> Equality.sort list
+
+        val elements_ge : Equality.sort -> SSAVS.t -> Equality.sort list
+
+        val set_induction_max :
+          (SSAVS.t -> __ -> 'a1) -> (SSAVS.t -> SSAVS.t -> 'a1 ->
+          Equality.sort -> __ -> __ -> 'a1) -> SSAVS.t -> 'a1
+
+        val set_induction_min :
+          (SSAVS.t -> __ -> 'a1) -> (SSAVS.t -> SSAVS.t -> 'a1 ->
+          Equality.sort -> __ -> __ -> 'a1) -> SSAVS.t -> 'a1
+
+        val memP : SSAVS.elt -> SSAVS.t -> reflect
+
+        val equalP : SSAVS.t -> SSAVS.t -> reflect
+
+        val subsetP : SSAVS.t -> SSAVS.t -> reflect
+
+        val emptyP : SSAVS.t -> reflect
+
+        val disjoint : SSAVS.t -> SSAVS.t -> bool
+
+        val proper_subset : SSAVS.t -> SSAVS.t -> bool
+       end
+
+      module VMLemmas :
+       sig
+        module F :
+         sig
+          val eqb : Equality.sort -> Equality.sort -> bool
+
+          val coq_In_dec : 'a1 TypEnv.SSATE.t -> TypEnv.SSATE.key -> bool
+         end
+
+        module OP :
+         sig
+          module ME :
+           sig
+            module TO :
+             sig
+              type t = Equality.sort
+             end
+
+            module IsTO :
+             sig
+             end
+
+            module OrderTac :
+             sig
+             end
+
+            val eq_dec : Equality.sort -> Equality.sort -> bool
+
+            val lt_dec : Equality.sort -> Equality.sort -> bool
+
+            val eqb : Equality.sort -> Equality.sort -> bool
+           end
+
+          module O :
+           sig
+            module MO :
+             sig
+              module TO :
+               sig
+                type t = Equality.sort
+               end
+
+              module IsTO :
+               sig
+               end
+
+              module OrderTac :
+               sig
+               end
+
+              val eq_dec : Equality.sort -> Equality.sort -> bool
+
+              val lt_dec : Equality.sort -> Equality.sort -> bool
+
+              val eqb : Equality.sort -> Equality.sort -> bool
+             end
+           end
+
+          module P :
+           sig
+            module F :
+             sig
+              val eqb : Equality.sort -> Equality.sort -> bool
+
+              val coq_In_dec : 'a1 TypEnv.SSATE.t -> TypEnv.SSATE.key -> bool
+             end
+
+            val uncurry : ('a1 -> 'a2 -> 'a3) -> ('a1 * 'a2) -> 'a3
+
+            val of_list : (TypEnv.SSATE.key * 'a1) list -> 'a1 TypEnv.SSATE.t
+
+            val to_list : 'a1 TypEnv.SSATE.t -> (TypEnv.SSATE.key * 'a1) list
+
+            val fold_rec :
+              (TypEnv.SSATE.key -> 'a1 -> 'a2 -> 'a2) -> 'a2 -> 'a1
+              TypEnv.SSATE.t -> ('a1 TypEnv.SSATE.t -> __ -> 'a3) ->
+              (TypEnv.SSATE.key -> 'a1 -> 'a2 -> 'a1 TypEnv.SSATE.t -> 'a1
+              TypEnv.SSATE.t -> __ -> __ -> __ -> 'a3 -> 'a3) -> 'a3
+
+            val fold_rec_bis :
+              (TypEnv.SSATE.key -> 'a1 -> 'a2 -> 'a2) -> 'a2 -> 'a1
+              TypEnv.SSATE.t -> ('a1 TypEnv.SSATE.t -> 'a1 TypEnv.SSATE.t ->
+              'a2 -> __ -> 'a3 -> 'a3) -> 'a3 -> (TypEnv.SSATE.key -> 'a1 ->
+              'a2 -> 'a1 TypEnv.SSATE.t -> __ -> __ -> 'a3 -> 'a3) -> 'a3
+
+            val fold_rec_nodep :
+              (TypEnv.SSATE.key -> 'a1 -> 'a2 -> 'a2) -> 'a2 -> 'a1
+              TypEnv.SSATE.t -> 'a3 -> (TypEnv.SSATE.key -> 'a1 -> 'a2 -> __
+              -> 'a3 -> 'a3) -> 'a3
+
+            val fold_rec_weak :
+              (TypEnv.SSATE.key -> 'a1 -> 'a2 -> 'a2) -> 'a2 -> ('a1
+              TypEnv.SSATE.t -> 'a1 TypEnv.SSATE.t -> 'a2 -> __ -> 'a3 ->
+              'a3) -> 'a3 -> (TypEnv.SSATE.key -> 'a1 -> 'a2 -> 'a1
+              TypEnv.SSATE.t -> __ -> 'a3 -> 'a3) -> 'a1 TypEnv.SSATE.t -> 'a3
+
+            val fold_rel :
+              (TypEnv.SSATE.key -> 'a1 -> 'a2 -> 'a2) -> (TypEnv.SSATE.key ->
+              'a1 -> 'a3 -> 'a3) -> 'a2 -> 'a3 -> 'a1 TypEnv.SSATE.t -> 'a4
+              -> (TypEnv.SSATE.key -> 'a1 -> 'a2 -> 'a3 -> __ -> 'a4 -> 'a4)
+              -> 'a4
+
+            val map_induction :
+              ('a1 TypEnv.SSATE.t -> __ -> 'a2) -> ('a1 TypEnv.SSATE.t -> 'a1
+              TypEnv.SSATE.t -> 'a2 -> TypEnv.SSATE.key -> 'a1 -> __ -> __ ->
+              'a2) -> 'a1 TypEnv.SSATE.t -> 'a2
+
+            val map_induction_bis :
+              ('a1 TypEnv.SSATE.t -> 'a1 TypEnv.SSATE.t -> __ -> 'a2 -> 'a2)
+              -> 'a2 -> (TypEnv.SSATE.key -> 'a1 -> 'a1 TypEnv.SSATE.t -> __
+              -> 'a2 -> 'a2) -> 'a1 TypEnv.SSATE.t -> 'a2
+
+            val cardinal_inv_2 :
+              'a1 TypEnv.SSATE.t -> int -> (TypEnv.SSATE.key * 'a1)
+
+            val cardinal_inv_2b :
+              'a1 TypEnv.SSATE.t -> (TypEnv.SSATE.key * 'a1)
+
+            val filter :
+              (TypEnv.SSATE.key -> 'a1 -> bool) -> 'a1 TypEnv.SSATE.t -> 'a1
+              TypEnv.SSATE.t
+
+            val for_all :
+              (TypEnv.SSATE.key -> 'a1 -> bool) -> 'a1 TypEnv.SSATE.t -> bool
+
+            val exists_ :
+              (TypEnv.SSATE.key -> 'a1 -> bool) -> 'a1 TypEnv.SSATE.t -> bool
+
+            val partition :
+              (TypEnv.SSATE.key -> 'a1 -> bool) -> 'a1 TypEnv.SSATE.t -> 'a1
+              TypEnv.SSATE.t * 'a1 TypEnv.SSATE.t
+
+            val update :
+              'a1 TypEnv.SSATE.t -> 'a1 TypEnv.SSATE.t -> 'a1 TypEnv.SSATE.t
+
+            val restrict :
+              'a1 TypEnv.SSATE.t -> 'a1 TypEnv.SSATE.t -> 'a1 TypEnv.SSATE.t
+
+            val diff :
+              'a1 TypEnv.SSATE.t -> 'a1 TypEnv.SSATE.t -> 'a1 TypEnv.SSATE.t
+
+            val coq_Partition_In :
+              'a1 TypEnv.SSATE.t -> 'a1 TypEnv.SSATE.t -> 'a1 TypEnv.SSATE.t
+              -> TypEnv.SSATE.key -> bool
+
+            val update_dec :
+              'a1 TypEnv.SSATE.t -> 'a1 TypEnv.SSATE.t -> TypEnv.SSATE.key ->
+              'a1 -> bool
+
+            val filter_dom :
+              (TypEnv.SSATE.key -> bool) -> 'a1 TypEnv.SSATE.t -> 'a1
+              TypEnv.SSATE.t
+
+            val filter_range :
+              ('a1 -> bool) -> 'a1 TypEnv.SSATE.t -> 'a1 TypEnv.SSATE.t
+
+            val for_all_dom :
+              (TypEnv.SSATE.key -> bool) -> 'a1 TypEnv.SSATE.t -> bool
+
+            val for_all_range : ('a1 -> bool) -> 'a1 TypEnv.SSATE.t -> bool
+
+            val exists_dom :
+              (TypEnv.SSATE.key -> bool) -> 'a1 TypEnv.SSATE.t -> bool
+
+            val exists_range : ('a1 -> bool) -> 'a1 TypEnv.SSATE.t -> bool
+
+            val partition_dom :
+              (TypEnv.SSATE.key -> bool) -> 'a1 TypEnv.SSATE.t -> 'a1
+              TypEnv.SSATE.t * 'a1 TypEnv.SSATE.t
+
+            val partition_range :
+              ('a1 -> bool) -> 'a1 TypEnv.SSATE.t -> 'a1 TypEnv.SSATE.t * 'a1
+              TypEnv.SSATE.t
+           end
+
+          val gtb :
+            (TypEnv.SSATE.key * 'a1) -> (TypEnv.SSATE.key * 'a1) -> bool
+
+          val leb :
+            (TypEnv.SSATE.key * 'a1) -> (TypEnv.SSATE.key * 'a1) -> bool
+
+          val elements_lt :
+            (TypEnv.SSATE.key * 'a1) -> 'a1 TypEnv.SSATE.t ->
+            (TypEnv.SSATE.key * 'a1) list
+
+          val elements_ge :
+            (TypEnv.SSATE.key * 'a1) -> 'a1 TypEnv.SSATE.t ->
+            (TypEnv.SSATE.key * 'a1) list
+
+          val max_elt_aux :
+            (TypEnv.SSATE.key * 'a1) list -> (TypEnv.SSATE.key * 'a1) option
+
+          val max_elt : 'a1 TypEnv.SSATE.t -> (TypEnv.SSATE.key * 'a1) option
+
+          val min_elt : 'a1 TypEnv.SSATE.t -> (TypEnv.SSATE.key * 'a1) option
+
+          val map_induction_max :
+            ('a1 TypEnv.SSATE.t -> __ -> 'a2) -> ('a1 TypEnv.SSATE.t -> 'a1
+            TypEnv.SSATE.t -> 'a2 -> Equality.sort -> 'a1 -> __ -> __ -> 'a2)
+            -> 'a1 TypEnv.SSATE.t -> 'a2
+
+          val map_induction_min :
+            ('a1 TypEnv.SSATE.t -> __ -> 'a2) -> ('a1 TypEnv.SSATE.t -> 'a1
+            TypEnv.SSATE.t -> 'a2 -> Equality.sort -> 'a1 -> __ -> __ -> 'a2)
+            -> 'a1 TypEnv.SSATE.t -> 'a2
+         end
+
+        val eqb : Equality.sort -> Equality.sort -> bool
+
+        val coq_In_dec : 'a1 TypEnv.SSATE.t -> TypEnv.SSATE.key -> bool
+
+        module ME :
+         sig
+          module TO :
+           sig
+            type t = Equality.sort
+           end
+
+          module IsTO :
+           sig
+           end
+
+          module OrderTac :
+           sig
+           end
+
+          val eq_dec : Equality.sort -> Equality.sort -> bool
+
+          val lt_dec : Equality.sort -> Equality.sort -> bool
+
+          val eqb : Equality.sort -> Equality.sort -> bool
+         end
+
+        module O :
+         sig
+          module MO :
+           sig
+            module TO :
+             sig
+              type t = Equality.sort
+             end
+
+            module IsTO :
+             sig
+             end
+
+            module OrderTac :
+             sig
+             end
+
+            val eq_dec : Equality.sort -> Equality.sort -> bool
+
+            val lt_dec : Equality.sort -> Equality.sort -> bool
+
+            val eqb : Equality.sort -> Equality.sort -> bool
+           end
+         end
+
+        module P :
+         sig
+          module F :
+           sig
+            val eqb : Equality.sort -> Equality.sort -> bool
+
+            val coq_In_dec : 'a1 TypEnv.SSATE.t -> TypEnv.SSATE.key -> bool
+           end
+
+          val uncurry : ('a1 -> 'a2 -> 'a3) -> ('a1 * 'a2) -> 'a3
+
+          val of_list : (TypEnv.SSATE.key * 'a1) list -> 'a1 TypEnv.SSATE.t
+
+          val to_list : 'a1 TypEnv.SSATE.t -> (TypEnv.SSATE.key * 'a1) list
+
+          val fold_rec :
+            (TypEnv.SSATE.key -> 'a1 -> 'a2 -> 'a2) -> 'a2 -> 'a1
+            TypEnv.SSATE.t -> ('a1 TypEnv.SSATE.t -> __ -> 'a3) ->
+            (TypEnv.SSATE.key -> 'a1 -> 'a2 -> 'a1 TypEnv.SSATE.t -> 'a1
+            TypEnv.SSATE.t -> __ -> __ -> __ -> 'a3 -> 'a3) -> 'a3
+
+          val fold_rec_bis :
+            (TypEnv.SSATE.key -> 'a1 -> 'a2 -> 'a2) -> 'a2 -> 'a1
+            TypEnv.SSATE.t -> ('a1 TypEnv.SSATE.t -> 'a1 TypEnv.SSATE.t ->
+            'a2 -> __ -> 'a3 -> 'a3) -> 'a3 -> (TypEnv.SSATE.key -> 'a1 ->
+            'a2 -> 'a1 TypEnv.SSATE.t -> __ -> __ -> 'a3 -> 'a3) -> 'a3
+
+          val fold_rec_nodep :
+            (TypEnv.SSATE.key -> 'a1 -> 'a2 -> 'a2) -> 'a2 -> 'a1
+            TypEnv.SSATE.t -> 'a3 -> (TypEnv.SSATE.key -> 'a1 -> 'a2 -> __ ->
+            'a3 -> 'a3) -> 'a3
+
+          val fold_rec_weak :
+            (TypEnv.SSATE.key -> 'a1 -> 'a2 -> 'a2) -> 'a2 -> ('a1
+            TypEnv.SSATE.t -> 'a1 TypEnv.SSATE.t -> 'a2 -> __ -> 'a3 -> 'a3)
+            -> 'a3 -> (TypEnv.SSATE.key -> 'a1 -> 'a2 -> 'a1 TypEnv.SSATE.t
+            -> __ -> 'a3 -> 'a3) -> 'a1 TypEnv.SSATE.t -> 'a3
+
+          val fold_rel :
+            (TypEnv.SSATE.key -> 'a1 -> 'a2 -> 'a2) -> (TypEnv.SSATE.key ->
+            'a1 -> 'a3 -> 'a3) -> 'a2 -> 'a3 -> 'a1 TypEnv.SSATE.t -> 'a4 ->
+            (TypEnv.SSATE.key -> 'a1 -> 'a2 -> 'a3 -> __ -> 'a4 -> 'a4) -> 'a4
+
+          val map_induction :
+            ('a1 TypEnv.SSATE.t -> __ -> 'a2) -> ('a1 TypEnv.SSATE.t -> 'a1
+            TypEnv.SSATE.t -> 'a2 -> TypEnv.SSATE.key -> 'a1 -> __ -> __ ->
+            'a2) -> 'a1 TypEnv.SSATE.t -> 'a2
+
+          val map_induction_bis :
+            ('a1 TypEnv.SSATE.t -> 'a1 TypEnv.SSATE.t -> __ -> 'a2 -> 'a2) ->
+            'a2 -> (TypEnv.SSATE.key -> 'a1 -> 'a1 TypEnv.SSATE.t -> __ ->
+            'a2 -> 'a2) -> 'a1 TypEnv.SSATE.t -> 'a2
+
+          val cardinal_inv_2 :
+            'a1 TypEnv.SSATE.t -> int -> (TypEnv.SSATE.key * 'a1)
+
+          val cardinal_inv_2b : 'a1 TypEnv.SSATE.t -> (TypEnv.SSATE.key * 'a1)
+
+          val filter :
+            (TypEnv.SSATE.key -> 'a1 -> bool) -> 'a1 TypEnv.SSATE.t -> 'a1
+            TypEnv.SSATE.t
+
+          val for_all :
+            (TypEnv.SSATE.key -> 'a1 -> bool) -> 'a1 TypEnv.SSATE.t -> bool
+
+          val exists_ :
+            (TypEnv.SSATE.key -> 'a1 -> bool) -> 'a1 TypEnv.SSATE.t -> bool
+
+          val partition :
+            (TypEnv.SSATE.key -> 'a1 -> bool) -> 'a1 TypEnv.SSATE.t -> 'a1
+            TypEnv.SSATE.t * 'a1 TypEnv.SSATE.t
+
+          val update :
+            'a1 TypEnv.SSATE.t -> 'a1 TypEnv.SSATE.t -> 'a1 TypEnv.SSATE.t
+
+          val restrict :
+            'a1 TypEnv.SSATE.t -> 'a1 TypEnv.SSATE.t -> 'a1 TypEnv.SSATE.t
+
+          val diff :
+            'a1 TypEnv.SSATE.t -> 'a1 TypEnv.SSATE.t -> 'a1 TypEnv.SSATE.t
+
+          val coq_Partition_In :
+            'a1 TypEnv.SSATE.t -> 'a1 TypEnv.SSATE.t -> 'a1 TypEnv.SSATE.t ->
+            TypEnv.SSATE.key -> bool
+
+          val update_dec :
+            'a1 TypEnv.SSATE.t -> 'a1 TypEnv.SSATE.t -> TypEnv.SSATE.key ->
+            'a1 -> bool
+
+          val filter_dom :
+            (TypEnv.SSATE.key -> bool) -> 'a1 TypEnv.SSATE.t -> 'a1
+            TypEnv.SSATE.t
+
+          val filter_range :
+            ('a1 -> bool) -> 'a1 TypEnv.SSATE.t -> 'a1 TypEnv.SSATE.t
+
+          val for_all_dom :
+            (TypEnv.SSATE.key -> bool) -> 'a1 TypEnv.SSATE.t -> bool
+
+          val for_all_range : ('a1 -> bool) -> 'a1 TypEnv.SSATE.t -> bool
+
+          val exists_dom :
+            (TypEnv.SSATE.key -> bool) -> 'a1 TypEnv.SSATE.t -> bool
+
+          val exists_range : ('a1 -> bool) -> 'a1 TypEnv.SSATE.t -> bool
+
+          val partition_dom :
+            (TypEnv.SSATE.key -> bool) -> 'a1 TypEnv.SSATE.t -> 'a1
+            TypEnv.SSATE.t * 'a1 TypEnv.SSATE.t
+
+          val partition_range :
+            ('a1 -> bool) -> 'a1 TypEnv.SSATE.t -> 'a1 TypEnv.SSATE.t * 'a1
+            TypEnv.SSATE.t
+         end
+
+        val gtb : (TypEnv.SSATE.key * 'a1) -> (TypEnv.SSATE.key * 'a1) -> bool
+
+        val leb : (TypEnv.SSATE.key * 'a1) -> (TypEnv.SSATE.key * 'a1) -> bool
+
+        val elements_lt :
+          (TypEnv.SSATE.key * 'a1) -> 'a1 TypEnv.SSATE.t ->
+          (TypEnv.SSATE.key * 'a1) list
+
+        val elements_ge :
+          (TypEnv.SSATE.key * 'a1) -> 'a1 TypEnv.SSATE.t ->
+          (TypEnv.SSATE.key * 'a1) list
+
+        val max_elt_aux :
+          (TypEnv.SSATE.key * 'a1) list -> (TypEnv.SSATE.key * 'a1) option
+
+        val max_elt : 'a1 TypEnv.SSATE.t -> (TypEnv.SSATE.key * 'a1) option
+
+        val min_elt : 'a1 TypEnv.SSATE.t -> (TypEnv.SSATE.key * 'a1) option
+
+        val map_induction_max :
+          ('a1 TypEnv.SSATE.t -> __ -> 'a2) -> ('a1 TypEnv.SSATE.t -> 'a1
+          TypEnv.SSATE.t -> 'a2 -> Equality.sort -> 'a1 -> __ -> __ -> 'a2)
+          -> 'a1 TypEnv.SSATE.t -> 'a2
+
+        val map_induction_min :
+          ('a1 TypEnv.SSATE.t -> __ -> 'a2) -> ('a1 TypEnv.SSATE.t -> 'a1
+          TypEnv.SSATE.t -> 'a2 -> Equality.sort -> 'a1 -> __ -> __ -> 'a2)
+          -> 'a1 TypEnv.SSATE.t -> 'a2
+
+        val memP : TypEnv.SSATE.key -> 'a1 TypEnv.SSATE.t -> reflect
+
+        val split :
+          ('a1 * 'a2) TypEnv.SSATE.t -> 'a1 TypEnv.SSATE.t * 'a2
+          TypEnv.SSATE.t
+
+        module EFacts :
+         sig
+          module TO :
+           sig
+            type t = Equality.sort
+           end
+
+          module IsTO :
+           sig
+           end
+
+          module OrderTac :
+           sig
+           end
+
+          val eq_dec : Equality.sort -> Equality.sort -> bool
+
+          val lt_dec : Equality.sort -> Equality.sort -> bool
+
+          val eqb : Equality.sort -> Equality.sort -> bool
+         end
+
+        val max_opt :
+          TypEnv.SSATE.key -> TypEnv.SSATE.key option -> TypEnv.SSATE.key
+
+        val max_key_elements :
+          (TypEnv.SSATE.key * 'a1) list -> TypEnv.SSATE.key option
+
+        val max_key : 'a1 TypEnv.SSATE.t -> TypEnv.SSATE.key option
+
+        val min_opt :
+          TypEnv.SSATE.key -> TypEnv.SSATE.key option -> TypEnv.SSATE.key
+
+        val min_key_elements :
+          (TypEnv.SSATE.key * 'a1) list -> TypEnv.SSATE.key option
+
+        val min_key : 'a1 TypEnv.SSATE.t -> TypEnv.SSATE.key option
+       end
+     end
+
+    module VSLemmas :
+     sig
+      module F :
+       sig
+        val eqb : Equality.sort -> Equality.sort -> bool
+       end
+
+      module OP :
+       sig
+        module ME :
+         sig
+          module TO :
+           sig
+            type t = Equality.sort
+           end
+
+          module IsTO :
+           sig
+           end
+
+          module OrderTac :
+           sig
+           end
+
+          val eq_dec : Equality.sort -> Equality.sort -> bool
+
+          val lt_dec : Equality.sort -> Equality.sort -> bool
+
+          val eqb : Equality.sort -> Equality.sort -> bool
+         end
+
+        module P :
+         sig
+          module Dec :
+           sig
+            module F :
+             sig
+              val eqb : Equality.sort -> Equality.sort -> bool
+             end
+
+            module FSetLogicalFacts :
+             sig
+             end
+
+            module FSetDecideAuxiliary :
+             sig
+             end
+
+            module FSetDecideTestCases :
+             sig
+             end
+           end
+
+          module FM :
+           sig
+            val eqb : Equality.sort -> Equality.sort -> bool
+           end
+
+          val coq_In_dec : SSAVS.elt -> SSAVS.t -> bool
+
+          val of_list : SSAVS.elt list -> SSAVS.t
+
+          val to_list : SSAVS.t -> SSAVS.elt list
+
+          val fold_rec :
+            (SSAVS.elt -> 'a1 -> 'a1) -> 'a1 -> SSAVS.t -> (SSAVS.t -> __ ->
+            'a2) -> (SSAVS.elt -> 'a1 -> SSAVS.t -> SSAVS.t -> __ -> __ -> __
+            -> 'a2 -> 'a2) -> 'a2
+
+          val fold_rec_bis :
+            (SSAVS.elt -> 'a1 -> 'a1) -> 'a1 -> SSAVS.t -> (SSAVS.t ->
+            SSAVS.t -> 'a1 -> __ -> 'a2 -> 'a2) -> 'a2 -> (SSAVS.elt -> 'a1
+            -> SSAVS.t -> __ -> __ -> 'a2 -> 'a2) -> 'a2
+
+          val fold_rec_nodep :
+            (SSAVS.elt -> 'a1 -> 'a1) -> 'a1 -> SSAVS.t -> 'a2 -> (SSAVS.elt
+            -> 'a1 -> __ -> 'a2 -> 'a2) -> 'a2
+
+          val fold_rec_weak :
+            (SSAVS.elt -> 'a1 -> 'a1) -> 'a1 -> (SSAVS.t -> SSAVS.t -> 'a1 ->
+            __ -> 'a2 -> 'a2) -> 'a2 -> (SSAVS.elt -> 'a1 -> SSAVS.t -> __ ->
+            'a2 -> 'a2) -> SSAVS.t -> 'a2
+
+          val fold_rel :
+            (SSAVS.elt -> 'a1 -> 'a1) -> (SSAVS.elt -> 'a2 -> 'a2) -> 'a1 ->
+            'a2 -> SSAVS.t -> 'a3 -> (SSAVS.elt -> 'a1 -> 'a2 -> __ -> 'a3 ->
+            'a3) -> 'a3
+
+          val set_induction :
+            (SSAVS.t -> __ -> 'a1) -> (SSAVS.t -> SSAVS.t -> 'a1 -> SSAVS.elt
+            -> __ -> __ -> 'a1) -> SSAVS.t -> 'a1
+
+          val set_induction_bis :
+            (SSAVS.t -> SSAVS.t -> __ -> 'a1 -> 'a1) -> 'a1 -> (SSAVS.elt ->
+            SSAVS.t -> __ -> 'a1 -> 'a1) -> SSAVS.t -> 'a1
+
+          val cardinal_inv_2 : SSAVS.t -> int -> SSAVS.elt
+
+          val cardinal_inv_2b : SSAVS.t -> SSAVS.elt
+         end
+
+        val gtb : Equality.sort -> Equality.sort -> bool
+
+        val leb : Equality.sort -> Equality.sort -> bool
+
+        val elements_lt : Equality.sort -> SSAVS.t -> Equality.sort list
+
+        val elements_ge : Equality.sort -> SSAVS.t -> Equality.sort list
+
+        val set_induction_max :
+          (SSAVS.t -> __ -> 'a1) -> (SSAVS.t -> SSAVS.t -> 'a1 ->
+          Equality.sort -> __ -> __ -> 'a1) -> SSAVS.t -> 'a1
+
+        val set_induction_min :
+          (SSAVS.t -> __ -> 'a1) -> (SSAVS.t -> SSAVS.t -> 'a1 ->
+          Equality.sort -> __ -> __ -> 'a1) -> SSAVS.t -> 'a1
+       end
+
+      val eqb : Equality.sort -> Equality.sort -> bool
+
+      module ME :
+       sig
+        module TO :
+         sig
+          type t = Equality.sort
+         end
+
+        module IsTO :
+         sig
+         end
+
+        module OrderTac :
+         sig
+         end
+
+        val eq_dec : Equality.sort -> Equality.sort -> bool
+
+        val lt_dec : Equality.sort -> Equality.sort -> bool
+
+        val eqb : Equality.sort -> Equality.sort -> bool
+       end
+
+      module P :
+       sig
+        module Dec :
+         sig
+          module F :
+           sig
+            val eqb : Equality.sort -> Equality.sort -> bool
+           end
+
+          module FSetLogicalFacts :
+           sig
+           end
+
+          module FSetDecideAuxiliary :
+           sig
+           end
+
+          module FSetDecideTestCases :
+           sig
+           end
+         end
+
+        module FM :
+         sig
+          val eqb : Equality.sort -> Equality.sort -> bool
+         end
+
+        val coq_In_dec : SSAVS.elt -> SSAVS.t -> bool
+
+        val of_list : SSAVS.elt list -> SSAVS.t
+
+        val to_list : SSAVS.t -> SSAVS.elt list
+
+        val fold_rec :
+          (SSAVS.elt -> 'a1 -> 'a1) -> 'a1 -> SSAVS.t -> (SSAVS.t -> __ ->
+          'a2) -> (SSAVS.elt -> 'a1 -> SSAVS.t -> SSAVS.t -> __ -> __ -> __
+          -> 'a2 -> 'a2) -> 'a2
+
+        val fold_rec_bis :
+          (SSAVS.elt -> 'a1 -> 'a1) -> 'a1 -> SSAVS.t -> (SSAVS.t -> SSAVS.t
+          -> 'a1 -> __ -> 'a2 -> 'a2) -> 'a2 -> (SSAVS.elt -> 'a1 -> SSAVS.t
+          -> __ -> __ -> 'a2 -> 'a2) -> 'a2
+
+        val fold_rec_nodep :
+          (SSAVS.elt -> 'a1 -> 'a1) -> 'a1 -> SSAVS.t -> 'a2 -> (SSAVS.elt ->
+          'a1 -> __ -> 'a2 -> 'a2) -> 'a2
+
+        val fold_rec_weak :
+          (SSAVS.elt -> 'a1 -> 'a1) -> 'a1 -> (SSAVS.t -> SSAVS.t -> 'a1 ->
+          __ -> 'a2 -> 'a2) -> 'a2 -> (SSAVS.elt -> 'a1 -> SSAVS.t -> __ ->
+          'a2 -> 'a2) -> SSAVS.t -> 'a2
+
+        val fold_rel :
+          (SSAVS.elt -> 'a1 -> 'a1) -> (SSAVS.elt -> 'a2 -> 'a2) -> 'a1 ->
+          'a2 -> SSAVS.t -> 'a3 -> (SSAVS.elt -> 'a1 -> 'a2 -> __ -> 'a3 ->
+          'a3) -> 'a3
+
+        val set_induction :
+          (SSAVS.t -> __ -> 'a1) -> (SSAVS.t -> SSAVS.t -> 'a1 -> SSAVS.elt
+          -> __ -> __ -> 'a1) -> SSAVS.t -> 'a1
+
+        val set_induction_bis :
+          (SSAVS.t -> SSAVS.t -> __ -> 'a1 -> 'a1) -> 'a1 -> (SSAVS.elt ->
+          SSAVS.t -> __ -> 'a1 -> 'a1) -> SSAVS.t -> 'a1
+
+        val cardinal_inv_2 : SSAVS.t -> int -> SSAVS.elt
+
+        val cardinal_inv_2b : SSAVS.t -> SSAVS.elt
+       end
+
+      val gtb : Equality.sort -> Equality.sort -> bool
+
+      val leb : Equality.sort -> Equality.sort -> bool
+
+      val elements_lt : Equality.sort -> SSAVS.t -> Equality.sort list
+
+      val elements_ge : Equality.sort -> SSAVS.t -> Equality.sort list
+
+      val set_induction_max :
+        (SSAVS.t -> __ -> 'a1) -> (SSAVS.t -> SSAVS.t -> 'a1 -> Equality.sort
+        -> __ -> __ -> 'a1) -> SSAVS.t -> 'a1
+
+      val set_induction_min :
+        (SSAVS.t -> __ -> 'a1) -> (SSAVS.t -> SSAVS.t -> 'a1 -> Equality.sort
+        -> __ -> __ -> 'a1) -> SSAVS.t -> 'a1
+
+      val memP : SSAVS.elt -> SSAVS.t -> reflect
+
+      val equalP : SSAVS.t -> SSAVS.t -> reflect
+
+      val subsetP : SSAVS.t -> SSAVS.t -> reflect
+
+      val emptyP : SSAVS.t -> reflect
+
+      val disjoint : SSAVS.t -> SSAVS.t -> bool
+
+      val proper_subset : SSAVS.t -> SSAVS.t -> bool
+     end
+
+    module VMLemmas :
+     sig
+      module F :
+       sig
+        val eqb : Equality.sort -> Equality.sort -> bool
+
+        val coq_In_dec : 'a1 TypEnv.SSATE.t -> TypEnv.SSATE.key -> bool
+       end
+
+      module OP :
+       sig
+        module ME :
+         sig
+          module TO :
+           sig
+            type t = Equality.sort
+           end
+
+          module IsTO :
+           sig
+           end
+
+          module OrderTac :
+           sig
+           end
+
+          val eq_dec : Equality.sort -> Equality.sort -> bool
+
+          val lt_dec : Equality.sort -> Equality.sort -> bool
+
+          val eqb : Equality.sort -> Equality.sort -> bool
+         end
+
+        module O :
+         sig
+          module MO :
+           sig
+            module TO :
+             sig
+              type t = Equality.sort
+             end
+
+            module IsTO :
+             sig
+             end
+
+            module OrderTac :
+             sig
+             end
+
+            val eq_dec : Equality.sort -> Equality.sort -> bool
+
+            val lt_dec : Equality.sort -> Equality.sort -> bool
+
+            val eqb : Equality.sort -> Equality.sort -> bool
+           end
+         end
+
+        module P :
+         sig
+          module F :
+           sig
+            val eqb : Equality.sort -> Equality.sort -> bool
+
+            val coq_In_dec : 'a1 TypEnv.SSATE.t -> TypEnv.SSATE.key -> bool
+           end
+
+          val uncurry : ('a1 -> 'a2 -> 'a3) -> ('a1 * 'a2) -> 'a3
+
+          val of_list : (TypEnv.SSATE.key * 'a1) list -> 'a1 TypEnv.SSATE.t
+
+          val to_list : 'a1 TypEnv.SSATE.t -> (TypEnv.SSATE.key * 'a1) list
+
+          val fold_rec :
+            (TypEnv.SSATE.key -> 'a1 -> 'a2 -> 'a2) -> 'a2 -> 'a1
+            TypEnv.SSATE.t -> ('a1 TypEnv.SSATE.t -> __ -> 'a3) ->
+            (TypEnv.SSATE.key -> 'a1 -> 'a2 -> 'a1 TypEnv.SSATE.t -> 'a1
+            TypEnv.SSATE.t -> __ -> __ -> __ -> 'a3 -> 'a3) -> 'a3
+
+          val fold_rec_bis :
+            (TypEnv.SSATE.key -> 'a1 -> 'a2 -> 'a2) -> 'a2 -> 'a1
+            TypEnv.SSATE.t -> ('a1 TypEnv.SSATE.t -> 'a1 TypEnv.SSATE.t ->
+            'a2 -> __ -> 'a3 -> 'a3) -> 'a3 -> (TypEnv.SSATE.key -> 'a1 ->
+            'a2 -> 'a1 TypEnv.SSATE.t -> __ -> __ -> 'a3 -> 'a3) -> 'a3
+
+          val fold_rec_nodep :
+            (TypEnv.SSATE.key -> 'a1 -> 'a2 -> 'a2) -> 'a2 -> 'a1
+            TypEnv.SSATE.t -> 'a3 -> (TypEnv.SSATE.key -> 'a1 -> 'a2 -> __ ->
+            'a3 -> 'a3) -> 'a3
+
+          val fold_rec_weak :
+            (TypEnv.SSATE.key -> 'a1 -> 'a2 -> 'a2) -> 'a2 -> ('a1
+            TypEnv.SSATE.t -> 'a1 TypEnv.SSATE.t -> 'a2 -> __ -> 'a3 -> 'a3)
+            -> 'a3 -> (TypEnv.SSATE.key -> 'a1 -> 'a2 -> 'a1 TypEnv.SSATE.t
+            -> __ -> 'a3 -> 'a3) -> 'a1 TypEnv.SSATE.t -> 'a3
+
+          val fold_rel :
+            (TypEnv.SSATE.key -> 'a1 -> 'a2 -> 'a2) -> (TypEnv.SSATE.key ->
+            'a1 -> 'a3 -> 'a3) -> 'a2 -> 'a3 -> 'a1 TypEnv.SSATE.t -> 'a4 ->
+            (TypEnv.SSATE.key -> 'a1 -> 'a2 -> 'a3 -> __ -> 'a4 -> 'a4) -> 'a4
+
+          val map_induction :
+            ('a1 TypEnv.SSATE.t -> __ -> 'a2) -> ('a1 TypEnv.SSATE.t -> 'a1
+            TypEnv.SSATE.t -> 'a2 -> TypEnv.SSATE.key -> 'a1 -> __ -> __ ->
+            'a2) -> 'a1 TypEnv.SSATE.t -> 'a2
+
+          val map_induction_bis :
+            ('a1 TypEnv.SSATE.t -> 'a1 TypEnv.SSATE.t -> __ -> 'a2 -> 'a2) ->
+            'a2 -> (TypEnv.SSATE.key -> 'a1 -> 'a1 TypEnv.SSATE.t -> __ ->
+            'a2 -> 'a2) -> 'a1 TypEnv.SSATE.t -> 'a2
+
+          val cardinal_inv_2 :
+            'a1 TypEnv.SSATE.t -> int -> (TypEnv.SSATE.key * 'a1)
+
+          val cardinal_inv_2b : 'a1 TypEnv.SSATE.t -> (TypEnv.SSATE.key * 'a1)
+
+          val filter :
+            (TypEnv.SSATE.key -> 'a1 -> bool) -> 'a1 TypEnv.SSATE.t -> 'a1
+            TypEnv.SSATE.t
+
+          val for_all :
+            (TypEnv.SSATE.key -> 'a1 -> bool) -> 'a1 TypEnv.SSATE.t -> bool
+
+          val exists_ :
+            (TypEnv.SSATE.key -> 'a1 -> bool) -> 'a1 TypEnv.SSATE.t -> bool
+
+          val partition :
+            (TypEnv.SSATE.key -> 'a1 -> bool) -> 'a1 TypEnv.SSATE.t -> 'a1
+            TypEnv.SSATE.t * 'a1 TypEnv.SSATE.t
+
+          val update :
+            'a1 TypEnv.SSATE.t -> 'a1 TypEnv.SSATE.t -> 'a1 TypEnv.SSATE.t
+
+          val restrict :
+            'a1 TypEnv.SSATE.t -> 'a1 TypEnv.SSATE.t -> 'a1 TypEnv.SSATE.t
+
+          val diff :
+            'a1 TypEnv.SSATE.t -> 'a1 TypEnv.SSATE.t -> 'a1 TypEnv.SSATE.t
+
+          val coq_Partition_In :
+            'a1 TypEnv.SSATE.t -> 'a1 TypEnv.SSATE.t -> 'a1 TypEnv.SSATE.t ->
+            TypEnv.SSATE.key -> bool
+
+          val update_dec :
+            'a1 TypEnv.SSATE.t -> 'a1 TypEnv.SSATE.t -> TypEnv.SSATE.key ->
+            'a1 -> bool
+
+          val filter_dom :
+            (TypEnv.SSATE.key -> bool) -> 'a1 TypEnv.SSATE.t -> 'a1
+            TypEnv.SSATE.t
+
+          val filter_range :
+            ('a1 -> bool) -> 'a1 TypEnv.SSATE.t -> 'a1 TypEnv.SSATE.t
+
+          val for_all_dom :
+            (TypEnv.SSATE.key -> bool) -> 'a1 TypEnv.SSATE.t -> bool
+
+          val for_all_range : ('a1 -> bool) -> 'a1 TypEnv.SSATE.t -> bool
+
+          val exists_dom :
+            (TypEnv.SSATE.key -> bool) -> 'a1 TypEnv.SSATE.t -> bool
+
+          val exists_range : ('a1 -> bool) -> 'a1 TypEnv.SSATE.t -> bool
+
+          val partition_dom :
+            (TypEnv.SSATE.key -> bool) -> 'a1 TypEnv.SSATE.t -> 'a1
+            TypEnv.SSATE.t * 'a1 TypEnv.SSATE.t
+
+          val partition_range :
+            ('a1 -> bool) -> 'a1 TypEnv.SSATE.t -> 'a1 TypEnv.SSATE.t * 'a1
+            TypEnv.SSATE.t
+         end
+
+        val gtb : (TypEnv.SSATE.key * 'a1) -> (TypEnv.SSATE.key * 'a1) -> bool
+
+        val leb : (TypEnv.SSATE.key * 'a1) -> (TypEnv.SSATE.key * 'a1) -> bool
+
+        val elements_lt :
+          (TypEnv.SSATE.key * 'a1) -> 'a1 TypEnv.SSATE.t ->
+          (TypEnv.SSATE.key * 'a1) list
+
+        val elements_ge :
+          (TypEnv.SSATE.key * 'a1) -> 'a1 TypEnv.SSATE.t ->
+          (TypEnv.SSATE.key * 'a1) list
+
+        val max_elt_aux :
+          (TypEnv.SSATE.key * 'a1) list -> (TypEnv.SSATE.key * 'a1) option
+
+        val max_elt : 'a1 TypEnv.SSATE.t -> (TypEnv.SSATE.key * 'a1) option
+
+        val min_elt : 'a1 TypEnv.SSATE.t -> (TypEnv.SSATE.key * 'a1) option
+
+        val map_induction_max :
+          ('a1 TypEnv.SSATE.t -> __ -> 'a2) -> ('a1 TypEnv.SSATE.t -> 'a1
+          TypEnv.SSATE.t -> 'a2 -> Equality.sort -> 'a1 -> __ -> __ -> 'a2)
+          -> 'a1 TypEnv.SSATE.t -> 'a2
+
+        val map_induction_min :
+          ('a1 TypEnv.SSATE.t -> __ -> 'a2) -> ('a1 TypEnv.SSATE.t -> 'a1
+          TypEnv.SSATE.t -> 'a2 -> Equality.sort -> 'a1 -> __ -> __ -> 'a2)
+          -> 'a1 TypEnv.SSATE.t -> 'a2
+       end
+
+      val eqb : Equality.sort -> Equality.sort -> bool
+
+      val coq_In_dec : 'a1 TypEnv.SSATE.t -> TypEnv.SSATE.key -> bool
+
+      module ME :
+       sig
+        module TO :
+         sig
+          type t = Equality.sort
+         end
+
+        module IsTO :
+         sig
+         end
+
+        module OrderTac :
+         sig
+         end
+
+        val eq_dec : Equality.sort -> Equality.sort -> bool
+
+        val lt_dec : Equality.sort -> Equality.sort -> bool
+
+        val eqb : Equality.sort -> Equality.sort -> bool
+       end
+
+      module O :
+       sig
+        module MO :
+         sig
+          module TO :
+           sig
+            type t = Equality.sort
+           end
+
+          module IsTO :
+           sig
+           end
+
+          module OrderTac :
+           sig
+           end
+
+          val eq_dec : Equality.sort -> Equality.sort -> bool
+
+          val lt_dec : Equality.sort -> Equality.sort -> bool
+
+          val eqb : Equality.sort -> Equality.sort -> bool
+         end
+       end
+
+      module P :
+       sig
+        module F :
+         sig
+          val eqb : Equality.sort -> Equality.sort -> bool
+
+          val coq_In_dec : 'a1 TypEnv.SSATE.t -> TypEnv.SSATE.key -> bool
+         end
+
+        val uncurry : ('a1 -> 'a2 -> 'a3) -> ('a1 * 'a2) -> 'a3
+
+        val of_list : (TypEnv.SSATE.key * 'a1) list -> 'a1 TypEnv.SSATE.t
+
+        val to_list : 'a1 TypEnv.SSATE.t -> (TypEnv.SSATE.key * 'a1) list
+
+        val fold_rec :
+          (TypEnv.SSATE.key -> 'a1 -> 'a2 -> 'a2) -> 'a2 -> 'a1
+          TypEnv.SSATE.t -> ('a1 TypEnv.SSATE.t -> __ -> 'a3) ->
+          (TypEnv.SSATE.key -> 'a1 -> 'a2 -> 'a1 TypEnv.SSATE.t -> 'a1
+          TypEnv.SSATE.t -> __ -> __ -> __ -> 'a3 -> 'a3) -> 'a3
+
+        val fold_rec_bis :
+          (TypEnv.SSATE.key -> 'a1 -> 'a2 -> 'a2) -> 'a2 -> 'a1
+          TypEnv.SSATE.t -> ('a1 TypEnv.SSATE.t -> 'a1 TypEnv.SSATE.t -> 'a2
+          -> __ -> 'a3 -> 'a3) -> 'a3 -> (TypEnv.SSATE.key -> 'a1 -> 'a2 ->
+          'a1 TypEnv.SSATE.t -> __ -> __ -> 'a3 -> 'a3) -> 'a3
+
+        val fold_rec_nodep :
+          (TypEnv.SSATE.key -> 'a1 -> 'a2 -> 'a2) -> 'a2 -> 'a1
+          TypEnv.SSATE.t -> 'a3 -> (TypEnv.SSATE.key -> 'a1 -> 'a2 -> __ ->
+          'a3 -> 'a3) -> 'a3
+
+        val fold_rec_weak :
+          (TypEnv.SSATE.key -> 'a1 -> 'a2 -> 'a2) -> 'a2 -> ('a1
+          TypEnv.SSATE.t -> 'a1 TypEnv.SSATE.t -> 'a2 -> __ -> 'a3 -> 'a3) ->
+          'a3 -> (TypEnv.SSATE.key -> 'a1 -> 'a2 -> 'a1 TypEnv.SSATE.t -> __
+          -> 'a3 -> 'a3) -> 'a1 TypEnv.SSATE.t -> 'a3
+
+        val fold_rel :
+          (TypEnv.SSATE.key -> 'a1 -> 'a2 -> 'a2) -> (TypEnv.SSATE.key -> 'a1
+          -> 'a3 -> 'a3) -> 'a2 -> 'a3 -> 'a1 TypEnv.SSATE.t -> 'a4 ->
+          (TypEnv.SSATE.key -> 'a1 -> 'a2 -> 'a3 -> __ -> 'a4 -> 'a4) -> 'a4
+
+        val map_induction :
+          ('a1 TypEnv.SSATE.t -> __ -> 'a2) -> ('a1 TypEnv.SSATE.t -> 'a1
+          TypEnv.SSATE.t -> 'a2 -> TypEnv.SSATE.key -> 'a1 -> __ -> __ ->
+          'a2) -> 'a1 TypEnv.SSATE.t -> 'a2
+
+        val map_induction_bis :
+          ('a1 TypEnv.SSATE.t -> 'a1 TypEnv.SSATE.t -> __ -> 'a2 -> 'a2) ->
+          'a2 -> (TypEnv.SSATE.key -> 'a1 -> 'a1 TypEnv.SSATE.t -> __ -> 'a2
+          -> 'a2) -> 'a1 TypEnv.SSATE.t -> 'a2
+
+        val cardinal_inv_2 :
+          'a1 TypEnv.SSATE.t -> int -> (TypEnv.SSATE.key * 'a1)
+
+        val cardinal_inv_2b : 'a1 TypEnv.SSATE.t -> (TypEnv.SSATE.key * 'a1)
+
+        val filter :
+          (TypEnv.SSATE.key -> 'a1 -> bool) -> 'a1 TypEnv.SSATE.t -> 'a1
+          TypEnv.SSATE.t
+
+        val for_all :
+          (TypEnv.SSATE.key -> 'a1 -> bool) -> 'a1 TypEnv.SSATE.t -> bool
+
+        val exists_ :
+          (TypEnv.SSATE.key -> 'a1 -> bool) -> 'a1 TypEnv.SSATE.t -> bool
+
+        val partition :
+          (TypEnv.SSATE.key -> 'a1 -> bool) -> 'a1 TypEnv.SSATE.t -> 'a1
+          TypEnv.SSATE.t * 'a1 TypEnv.SSATE.t
+
+        val update :
+          'a1 TypEnv.SSATE.t -> 'a1 TypEnv.SSATE.t -> 'a1 TypEnv.SSATE.t
+
+        val restrict :
+          'a1 TypEnv.SSATE.t -> 'a1 TypEnv.SSATE.t -> 'a1 TypEnv.SSATE.t
+
+        val diff :
+          'a1 TypEnv.SSATE.t -> 'a1 TypEnv.SSATE.t -> 'a1 TypEnv.SSATE.t
+
+        val coq_Partition_In :
+          'a1 TypEnv.SSATE.t -> 'a1 TypEnv.SSATE.t -> 'a1 TypEnv.SSATE.t ->
+          TypEnv.SSATE.key -> bool
+
+        val update_dec :
+          'a1 TypEnv.SSATE.t -> 'a1 TypEnv.SSATE.t -> TypEnv.SSATE.key -> 'a1
+          -> bool
+
+        val filter_dom :
+          (TypEnv.SSATE.key -> bool) -> 'a1 TypEnv.SSATE.t -> 'a1
+          TypEnv.SSATE.t
+
+        val filter_range :
+          ('a1 -> bool) -> 'a1 TypEnv.SSATE.t -> 'a1 TypEnv.SSATE.t
+
+        val for_all_dom :
+          (TypEnv.SSATE.key -> bool) -> 'a1 TypEnv.SSATE.t -> bool
+
+        val for_all_range : ('a1 -> bool) -> 'a1 TypEnv.SSATE.t -> bool
+
+        val exists_dom :
+          (TypEnv.SSATE.key -> bool) -> 'a1 TypEnv.SSATE.t -> bool
+
+        val exists_range : ('a1 -> bool) -> 'a1 TypEnv.SSATE.t -> bool
+
+        val partition_dom :
+          (TypEnv.SSATE.key -> bool) -> 'a1 TypEnv.SSATE.t -> 'a1
+          TypEnv.SSATE.t * 'a1 TypEnv.SSATE.t
+
+        val partition_range :
+          ('a1 -> bool) -> 'a1 TypEnv.SSATE.t -> 'a1 TypEnv.SSATE.t * 'a1
+          TypEnv.SSATE.t
+       end
+
+      val gtb : (TypEnv.SSATE.key * 'a1) -> (TypEnv.SSATE.key * 'a1) -> bool
+
+      val leb : (TypEnv.SSATE.key * 'a1) -> (TypEnv.SSATE.key * 'a1) -> bool
+
+      val elements_lt :
+        (TypEnv.SSATE.key * 'a1) -> 'a1 TypEnv.SSATE.t ->
+        (TypEnv.SSATE.key * 'a1) list
+
+      val elements_ge :
+        (TypEnv.SSATE.key * 'a1) -> 'a1 TypEnv.SSATE.t ->
+        (TypEnv.SSATE.key * 'a1) list
+
+      val max_elt_aux :
+        (TypEnv.SSATE.key * 'a1) list -> (TypEnv.SSATE.key * 'a1) option
+
+      val max_elt : 'a1 TypEnv.SSATE.t -> (TypEnv.SSATE.key * 'a1) option
+
+      val min_elt : 'a1 TypEnv.SSATE.t -> (TypEnv.SSATE.key * 'a1) option
+
+      val map_induction_max :
+        ('a1 TypEnv.SSATE.t -> __ -> 'a2) -> ('a1 TypEnv.SSATE.t -> 'a1
+        TypEnv.SSATE.t -> 'a2 -> Equality.sort -> 'a1 -> __ -> __ -> 'a2) ->
+        'a1 TypEnv.SSATE.t -> 'a2
+
+      val map_induction_min :
+        ('a1 TypEnv.SSATE.t -> __ -> 'a2) -> ('a1 TypEnv.SSATE.t -> 'a1
+        TypEnv.SSATE.t -> 'a2 -> Equality.sort -> 'a1 -> __ -> __ -> 'a2) ->
+        'a1 TypEnv.SSATE.t -> 'a2
+
+      val memP : TypEnv.SSATE.key -> 'a1 TypEnv.SSATE.t -> reflect
+
+      val split :
+        ('a1 * 'a2) TypEnv.SSATE.t -> 'a1 TypEnv.SSATE.t * 'a2 TypEnv.SSATE.t
+
+      module EFacts :
+       sig
+        module TO :
+         sig
+          type t = Equality.sort
+         end
+
+        module IsTO :
+         sig
+         end
+
+        module OrderTac :
+         sig
+         end
+
+        val eq_dec : Equality.sort -> Equality.sort -> bool
+
+        val lt_dec : Equality.sort -> Equality.sort -> bool
+
+        val eqb : Equality.sort -> Equality.sort -> bool
+       end
+
+      val max_opt :
+        TypEnv.SSATE.key -> TypEnv.SSATE.key option -> TypEnv.SSATE.key
+
+      val max_key_elements :
+        (TypEnv.SSATE.key * 'a1) list -> TypEnv.SSATE.key option
+
+      val max_key : 'a1 TypEnv.SSATE.t -> TypEnv.SSATE.key option
+
+      val min_opt :
+        TypEnv.SSATE.key -> TypEnv.SSATE.key option -> TypEnv.SSATE.key
+
+      val min_key_elements :
+        (TypEnv.SSATE.key * 'a1) list -> TypEnv.SSATE.key option
+
+      val min_key : 'a1 TypEnv.SSATE.t -> TypEnv.SSATE.key option
+     end
+   end
  end
 
 val eunop_eqType : Equality.coq_type
